Add in-progress proof of the fact that LL(1) grammars are unambiguous

LL1/ParseTable.v
@@ -41,12 +41,12 @@ Definition parseTableLookup
 
 (* Changed nullableSym from nonterminal to symbol *)
 Inductive nullableProd {g : grammar} :
-  nonterminal -> list symbol -> Prop :=
+  symbol -> list symbol -> Prop :=
 | NuProd :
     forall x ys,
       In (x, ys) g.(productions)
       -> nullableGamma ys
-      -> nullableProd x ys
+      -> nullableProd (NT x) ys
 with nullableGamma {g : grammar} :
        list symbol -> Prop :=
      | NuNil :
@@ -59,16 +59,16 @@ with nullableGamma {g : grammar} :
 with nullableSym {g : grammar} :
        symbol -> Prop :=
      | NuSym :
-         forall x ys,
-           nullableProd x ys
-           -> nullableSym (NT x).
+         forall sym ys,
+           nullableProd sym ys
+           -> nullableSym sym.
 
 Inductive firstProd {g : grammar} :
-    lookahead -> nonterminal -> list symbol -> Prop :=
+    lookahead -> symbol -> list symbol -> Prop :=
 | FiProd : forall la x gamma,
     In (x, gamma) g.(productions)
     -> firstGamma la gamma
-    -> firstProd la x gamma
+    -> firstProd la (NT x) gamma
 with firstGamma {g : grammar} :
        lookahead -> list symbol -> Prop :=
      | FiGammaHd : forall la hd tl,
@@ -82,216 +82,59 @@ with firstSym {g : grammar} :
        lookahead -> symbol -> Prop :=
 | FiT : forall s,
     firstSym (LA s) (T s)
-| FiNT : forall la x gamma,
-    firstProd la x gamma ->
-    firstSym la (NT x).
+| FiNT : forall la sym gamma,
+    firstProd la sym gamma ->
+    firstSym la sym.
 
 Scheme firstProd_mutual_ind := Induction for firstProd Sort Prop
   with firstGamma_mutual_ind := Induction for firstGamma Sort Prop
   with firstSym_mutual_ind := Induction for firstSym Sort Prop.
 
 Inductive followProd {g : grammar} :
-  lookahead -> nonterminal -> list symbol -> Prop :=
+  lookahead -> symbol -> list symbol -> Prop :=
 | FoProd :
     forall la x gamma,
       In (x, gamma) g.(productions)
-      -> followSym la x
-      -> followProd la x gamma
+      -> followSym la (NT x)
+      -> followProd la (NT x) gamma
 with followSym {g : grammar} :
-       lookahead -> nonterminal -> Prop :=
-     | FoStart :
-         followSym EOF g.(start)
+       lookahead -> symbol -> Prop :=
+     | FoNu :
+         forall sym gamma,
+           (@nullableProd g) sym gamma
+           -> followSym EOF sym
      | FoRight :
          forall x1 x2 prefix suffix la,
            In (x1, prefix ++ NT x2 :: suffix) g.(productions)
            -> (@firstGamma g) la suffix
-           -> followSym la x2
+           -> followSym la (NT x2)
      | FoLeft :
          forall x1 x2 prefix suffix la,
            In (x1, prefix ++ NT x2 :: suffix) g.(productions)
            -> (@nullableGamma g) suffix
-           -> followSym la x1
-           -> followSym la x2.
+           -> followSym la (NT x1)
+           -> followSym la (NT x2).
 
 Scheme followProd_mutual_ind := Induction for firstProd Sort Prop
   with followSym_mutual_ind := Induction for firstSym Sort Prop.
 
-Definition isLookaheadFor {g} la x gamma :=
-  (@firstProd g) la x gamma
-  \/ (@nullableProd g) x gamma /\ (@followProd g) la x gamma.
+Definition isLookaheadFor {g} la sym gamma :=
+  (@firstProd g) la sym gamma
+  \/ (@nullableProd g) sym gamma
+     /\ (@followProd g) la sym gamma.
 
 Definition ptMinimal tbl g :=
   forall x la gamma laMap,
     StringMap.find x tbl = Some laMap
     -> LookaheadMap.find la laMap = Some gamma
-    -> (@isLookaheadFor g) la x gamma.
+    -> (@isLookaheadFor g) la (NT x) gamma.
 
 Definition ptComplete tbl g :=
   forall x la gamma,
-    (@isLookaheadFor g) la x gamma
+    (@isLookaheadFor g) la (NT x) gamma
     -> exists laMap,
       StringMap.find x tbl = Some laMap
       /\ LookaheadMap.find la laMap = Some gamma.
 
 Definition isParseTableFor (tbl : parse_table) (g : grammar) :=
   ptMinimal tbl g /\ ptComplete tbl g.
-
-(*
-
-(* This can be simplified a little *)
-Inductive nullableSym {g : grammar} : nonterminal -> Prop :=
-| nullable_nt :
-    forall x gamma,
-      nullableProd x gamma ->
-      nullableSym x
-with nullableProd {g : grammar} : nonterminal -> list symbol -> Prop :=
-     | nprod :
-         forall x ys,
-           In (x, ys) g.(productions) ->
-           (forall sym,
-               In sym ys ->
-               sym <> NT x) ->
-           nullableGamma ys ->
-           nullableProd x ys
-with nullableGamma {g : grammar} : list symbol -> Prop :=
-     | nullable_nil :
-         nullableGamma nil
-     | nullable_cons :
-         forall hd tl,
-           nullableSym hd ->
-           nullableGamma tl ->
-           nullableGamma (NT hd :: tl).
-
-Definition nullableSetComplete (nu : StringSet.t)
-                               (g : grammar) : Prop :=
-  forall x,
-    (@nullableSym g) x ->
-    StringSet.In x nu.
-
-Definition nullableSetMinimal (nu : StringSet.t)
-                              (g  : grammar) : Prop :=
-  forall x,
-    StringSet.In x nu ->
-    (@nullableSym g) x.
-
-Definition isNullableSetFor nu g : Prop :=
-  nullableSetComplete nu g /\ nullableSetMinimal nu g.
-
-
-(* Definition of the FIRST set for a given grammar *)
-
-Inductive firstSym {g : grammar} :
-  lookahead -> symbol -> Prop :=
-| first_t : forall s,
-    firstSym (LA s) (T s)
-| first_nt : forall x y ys,
-    firstProd y x ys ->
-    firstSym y (NT x)
-with firstProd {g : grammar} :
-       lookahead -> nonterminal -> list symbol -> Prop :=
-     | fprod : forall y x ys,
-         In (x, ys) g.(productions) ->
-         firstProd' y x ys ->
-         firstProd y x ys
-with firstProd' {g : grammar} :
-       lookahead -> nonterminal -> list symbol -> Prop :=
-     | fprod_hd : forall y x hd tl,
-         NT x <> hd ->
-         firstSym y hd ->
-         firstProd' y x (hd :: tl)
-     | fprod_tl : forall y x hd tl,
-         (@nullableSym g) hd ->
-         firstProd' y x tl ->
-         firstProd' y x (NT hd :: tl).
-
-Inductive firstGamma {g : grammar} :
-  lookahead -> list symbol -> Prop :=
-| fgamma_hd : forall y hd tl,
-    (@firstSym g) y hd ->
-    firstGamma y (hd :: tl)
-| fgamma_tl : forall y hd tl,
-    (@nullableSym g) hd ->
-    firstGamma y tl ->
-    firstGamma y (NT hd :: tl).
-
-Definition firstSetComplete fi g : Prop :=
-  forall x y,
-    (@firstSym g) y (NT x) ->
-    exists xFirst,
-      StringMap.find x fi = Some xFirst /\
-      LookaheadSet.In y xFirst.
-
-Definition firstSetMinimal fi g : Prop :=
-  forall x xFirst y,
-    StringMap.find x fi = Some xFirst ->
-    LookaheadSet.In y xFirst ->
-    (@firstSym g) y (NT x).
-
-Definition isFirstSetFor fi g : Prop :=
-  firstSetComplete fi g /\ firstSetMinimal fi g.
-
-
-(* Definition of the FOLLOW set for a given grammar *)
-
-(* Remember to add EOF *)
-Inductive followSym {g : grammar} : lookahead -> nonterminal -> Prop :=
-| followRight :
-    forall lx rx prefix suffix y,
-      In (lx, (prefix ++ NT rx :: suffix)%list) g.(productions) ->
-      (@firstGamma g) y suffix -> 
-      followSym y rx
-| followLeft :
-    forall lx rx prefix suffix la,
-      In (lx, (prefix ++ NT rx :: suffix)%list) g.(productions) ->
-      lx <> rx -> (* Necessary? *)
-      (@nullableGamma g) suffix ->
-      followSym la lx ->
-      followSym la rx.
-
-Definition followSetComplete fo g : Prop :=
-  forall x y,
-    (@followSym g) y x ->
-    exists xFollow,
-      StringMap.find x fo = Some xFollow /\
-      LookaheadSet.In y xFollow.
-
-Definition followSetMinimal fo g : Prop :=
-  forall x xFollow y,
-    StringMap.find x fo = Some xFollow ->
-    LookaheadSet.In y xFollow ->
-    (@followSym g) y x.
-
-Definition isFollowSetFor fo g : Prop :=
-  followSetComplete fo g /\ followSetMinimal fo g.
-
-Definition ptCompleteFirst tbl g : Prop :=
-  forall x gamma y,
-    In (x, gamma) g.(productions) ->
-    (@firstGamma g) y gamma ->
-    exists tMap,
-      StringMap.find x tbl = Some tMap  /\
-      LookaheadMap.find y tMap = Some gamma. 
-
-Definition ptCompleteFollow tbl g : Prop :=
-  forall x gamma y,
-    In (x, gamma) g.(productions) ->
-    (@nullableGamma g) gamma ->
-    (@followSym g) y x ->
-    exists tMap,
-      StringMap.find x tbl  = Some tMap /\
-      LookaheadMap.find y tMap = Some gamma.
-
-Definition parseTableComplete tbl g : Prop :=
-  ptCompleteFirst tbl g /\ ptCompleteFollow tbl g.
-
-Definition parseTableMinimal tbl g : Prop :=
-  forall x tMap y gamma,
-    StringMap.find x tbl = Some tMap ->
-    LookaheadMap.find y tMap = Some gamma ->
-    (@firstProd g) y x gamma \/
-    (@nullableProd g) x gamma /\ (@followSym g) y x.
-
-Definition isParseTableFor tbl g : Prop :=
-  parseTableComplete tbl g /\ parseTableMinimal tbl g.
-
-*)
