Lib/ParseTree.v
@@ -1,4 +1,4 @@
-Require Import String.
+Require Import String List.
 Require Import Grammar.
 
 Inductive tree :=
@@ -7,6 +7,7 @@ Inductive tree :=
 with forest :=
      | Fnil : forest
      | Fcons : tree -> forest -> forest.
+
 
 Definition isNode (tr : tree) : bool :=
   match tr with
@@ -23,6 +24,36 @@ Scheme tree_mutual_ind := Induction for tree Sort Prop
 Combined Scheme tree_forest_mutual_ind
          from tree_mutual_ind, forest_mutual_ind.
 
+Section more_ind.
+
+  Variable P : tree -> Prop.
+  Variable Q : forest -> Prop.
+
+  Hypothesis H : forall s l, Q l -> P (Node s l).
+  Hypothesis H0 : Q Fnil.
+  Hypothesis H1 :
+    forall tr,
+      P tr
+      -> forall l,
+        Q l
+        -> Q (Fcons tr l).
+  Hypothesis H2 : forall y, P (Leaf y).
+
+  Import ListNotations.
+
+  Fixpoint tree_nested_ind t : P t :=
+    match t with
+    | Leaf y => H2 y
+    | Node x l =>
+      H x l
+        (((fix l_ind l' : Q l' :=
+             match l' with
+             | Fnil => H0
+             | Fcons t1 tl => H1 t1 (tree_nested_ind t1) tl (l_ind tl)
+             end)) l)
+    end.
+End more_ind.
+
 Fixpoint span tr :=
   match tr with
   | Leaf _ => 1
@@ -35,3 +66,44 @@ with spanForest f :=
        | Fcons hd tl =>
          span hd + spanForest tl
        end.
+
+Fixpoint All (f : forest) (P : tree -> Prop) : Prop :=
+  match f with
+  | Fnil => True
+  | Fcons tr f' => P tr /\ All f' P
+  end.
+
+Section tree2.
+
+  Inductive ptree :=
+  | PLeaf : string -> ptree
+  | PNode : string -> list ptree -> ptree.
+
+  Variable P : ptree -> Prop.
+  Variable Q : list ptree -> Prop.
+
+  Hypothesis H : forall s l, Q l -> P (PNode s l).
+  Hypothesis H0 : Q nil.
+  Hypothesis H1 :
+    forall tr,
+      P tr
+      -> forall l,
+        Q l
+        -> Q (tr :: l).
+  Hypothesis H2 : forall y, P (PLeaf y).
+
+  Import ListNotations.
+
+  Fixpoint ptree_ind' t : P t :=
+    match t with
+    | PLeaf y => H2 y
+    | PNode x l =>
+      H x l
+        (((fix l_ind l' : Q l' :=
+             match l' with
+             | nil => H0
+             | t1 :: tl => H1 t1 (ptree_ind' t1) tl (l_ind tl)
+             end)) l)
+    end.
+End tree2.
+
