LL1/DeterminismProof.v
@@ -1,0 +1,2671 @@
+Require Import List Omega String.
+Require Import Derivation Grammar Lemmas ParseTable Utils
+        ParseTree LL1.Parser Lib.Tactics
+        LL1.CorrectnessProof LL1.MonotonicityLemmas.
+Import ListNotations.
+Open Scope list_scope.
+
+
+Inductive derivesProd {g : grammar} :
+  nonterminal -> list symbol -> list string -> tree -> Prop :=
+| derProd :
+    forall x gamma tokens f,
+      In (x, gamma) g.(productions)
+      -> derivesGamma gamma tokens f
+      -> derivesProd x gamma tokens (Node x f)
+with derivesGamma {g : grammar} : 
+       list symbol -> list string -> forest -> Prop :=
+     | derivesFnil : derivesGamma [] [] Fnil
+     | derivesFcons : 
+         forall (hdSym : symbol)
+                (prefix suffix : list string)
+                (hdTree : tree)
+                (tlSyms : list symbol)
+                (tlTrees : forest),
+           derivesSym hdSym prefix hdTree
+         -> derivesGamma tlSyms suffix tlTrees
+         -> derivesGamma (hdSym :: tlSyms) 
+                         (prefix ++ suffix) 
+                         (Fcons hdTree tlTrees)
+with derivesSym {g : grammar} : 
+       symbol -> list string -> tree -> Prop :=
+     | derivesT : 
+         forall (y : string),
+           derivesSym (T y) [y] (Leaf y)
+     | derivesNT : 
+         forall (x : string) 
+                (gamma : list symbol) 
+                (tokens : list string) 
+                tr,
+           derivesProd x gamma tokens tr
+           -> derivesSym (NT x) tokens tr.
+
+Scheme derivesProd_mut_ind := Induction for derivesProd Sort Prop
+  with derivesGamma_mut_ind := Induction for derivesGamma Sort Prop
+  with derivesSym_mut_ind := Induction for derivesSym Sort Prop.
+
+
+Lemma derivesSym_nil_nullable :
+  forall tr g sym,
+    (@derivesSym g) sym [] tr
+    -> (@nullableSym g) sym.
+ Proof.
+  induction tr using tree_mutual_ind with
+      (P := fun tr =>
+              forall g sym,
+                (@derivesSym g) sym [] tr
+                -> (@nullableSym g) sym)
+      (P0 := fun f =>
+               forall g gamma,
+                 (@derivesGamma g) gamma nil f
+                 -> (@nullableGamma g) gamma).
+
+  - intros g sym Hder.
+    inv Hder.
+    inv H.
+
+  - intros g sym Hder.
+    inv Hder.
+    inv H.
+    econstructor.
+    econstructor.
+    + eauto.
+    + apply IHtr.
+      auto.
+
+  - intros g gamma Hder.
+    inv Hder.
+    constructor.
+
+  - intros g gamma Hder.
+    inv Hder.
+    assert (prefix = nil).
+    { destruct prefix; destruct suffix; try inv H; auto. }
+    assert (suffix = nil).
+    { destruct prefix; destruct suffix; try inv H; auto. }
+    subst.
+    clear H.
+    inv H3.
+    inv H.
+    constructor.
+    + apply IHtr.
+      econstructor.
+      econstructor; eauto.
+    + apply IHtr0.
+      auto.
+ Qed.
+
+ Lemma derivesGamma_nil_nullable :
+  forall f g gamma,
+    (@derivesGamma g) gamma [] f
+    -> (@nullableGamma g) gamma.
+ Proof.
+  induction f using forest_mutual_ind with
+      (P := fun tr =>
+              forall g sym,
+                (@derivesSym g) sym [] tr
+                -> (@nullableSym g) sym)
+      (P0 := fun f =>
+               forall g gamma,
+                 (@derivesGamma g) gamma nil f
+                 -> (@nullableGamma g) gamma).
+
+  - intros g sym Hder.
+    inv Hder.
+    inv H.
+
+  - intros g sym Hder.
+    inv Hder.
+    inv H.
+    econstructor.
+    econstructor.
+    + eauto.
+    + apply IHf.
+      auto.
+
+  - intros g gamma Hder.
+    inv Hder.
+    constructor.
+
+  - intros g gamma Hder.
+    inv Hder.
+    assert (prefix = nil).
+    { destruct prefix; destruct suffix; try inv H; auto. }
+    assert (suffix = nil).
+    { destruct prefix; destruct suffix; try inv H; auto. }
+    subst.
+    clear H.
+    inv H3.
+    inv H.
+    constructor.
+    + apply IHf.
+      econstructor.
+      econstructor; eauto.
+    + apply IHf0.
+      auto.
+ Qed.
+
+ (* to do *)
+ Lemma derivesGamma_cons_firstGamma :
+   forall f g tok toks gamma,
+     (@derivesGamma g) gamma (tok :: toks) f
+    -> (@firstGamma g) (LA tok) gamma.
+ Proof.
+ Admitted.
+
+ Fixpoint appF f f2 :=
+   match f with
+   | Fnil => f2
+   | Fcons tr f' => Fcons tr (appF f' f2)
+   end.
+
+Lemma appF_nil_r : forall f,
+    appF f Fnil = f.
+Proof.
+  induction f; simpl.
+  - auto.
+  - rewrite IHf. auto.
+Qed.
+
+Lemma appF_nil_l : forall f,
+    appF Fnil f = f.
+Proof.
+  intros. simpl. auto.
+Qed.
+
+Fixpoint lengthF f :=
+  match f with
+  | Fnil => 0
+  | Fcons t f' => 1 + lengthF f'
+  end.
+
+Lemma forest_length :
+  forall g gamma word f,
+    (@derivesGamma g) gamma word f
+    -> List.length gamma = lengthF f.
+Proof.
+  induction gamma; intros.
+  - inv H.
+    simpl.
+    auto.
+  - inv H.
+    simpl.
+    apply eq_S.
+    eapply IHgamma.
+    eauto.
+Qed.
+
+Lemma lengths_contra :
+  forall f tr f',
+    ~ lengthF f = lengthF (appF f (Fcons tr f')).
+Proof.
+  induction f; unfold not; intros.
+  - simpl in H.
+    inv H.
+  - unfold not in *.
+    simpl in *.
+    apply (IHf tr f').
+    auto.
+Qed.
+
+Lemma lengths_contra_l :
+  forall f f' tr,
+    ~ lengthF f = lengthF (appF (Fcons tr f') f).
+Proof.
+  induction f; unfold not in *; intros.
+  - simpl in H.
+    inv H.
+  - simpl in *.
+Admitted.
+
+Lemma appF_Fcons_not_Fnil :
+  forall f f' tr,
+    Fnil <> appF f (Fcons tr f').
+Proof.
+  destruct f; unfold not; intros; simpl in *.
+  - inv H.
+  - inv H.
+Qed.
+
+Lemma nullable_middle_sym :
+  forall g xs ys sym,
+    (@nullableGamma g) (xs ++ sym :: ys)
+    -> (@nullableSym g) sym.
+Proof.
+  induction xs; intros.
+  - simpl in H.
+    inv H.
+    auto.
+  - eapply IHxs.
+    inv H.
+    eauto.
+Qed.
+
+Lemma gamma_with_terminal_not_nullable :
+  forall g xs y zs,
+    (@nullableGamma g) (xs ++ T y :: zs)
+    -> False.
+Proof.
+  induction xs; intros.
+  - simpl in H.
+    inv H.
+  - destruct a.
+    + inv H.
+    + inv H.
+      eapply IHxs; eauto.
+Qed.
+
+Lemma nullable_split :
+  forall g xs ys,
+    (@nullableGamma g) (xs ++ ys)
+    -> (@nullableGamma g) ys.
+Proof.
+  induction xs; intros.
+  - auto.
+  - inv H.
+    eapply IHxs; eauto.
+Qed.
+  
+Lemma no_first_follow_conflicts :
+  forall tbl g,
+    isParseTableFor tbl g
+    -> forall la sym gamma,
+      (@firstProd g) la sym gamma
+      -> (@nullableProd g) sym gamma
+      -> (@followProd g) la sym gamma
+      -> False.
+Proof.
+  intros tbl g Htbl la sym gamma Hfi.
+  destruct Htbl as [Hmin Hcom].
+  induction Hfi using firstProd_mutual_ind with
+      (P := fun la sym gamma
+                (pf : (@firstProd g) la sym gamma) =>
+              (@nullableProd g) sym gamma
+              -> (@followProd g) la sym gamma
+              -> False)
+      (P0 := fun la gammaSuf
+                 (pf : (@firstGamma g) la gammaSuf) =>
+               forall sym gammaPre,
+                 (@firstProd g) la sym (gammaPre ++ gammaSuf)
+                 -> (@nullableProd g) sym (gammaPre ++ gammaSuf)
+                 -> (@followProd g) la sym (gammaPre ++ gammaSuf)
+                 -> False)
+      (P1 := fun la sym (pf : (@firstSym g) la sym) =>
+              (@nullableSym g) sym
+              -> (@followSym g) la sym
+              -> False).
+
+  - intros Hnu Hfo.
+    eapply IHHfi; auto.
+    + assert (gamma = [] ++ gamma) by auto.
+      rewrite H in i.
+      econstructor; eauto.
+    + auto.
+    + auto.
+
+  - intros sym gammaSuf Hfi Hnu Hfo.
+    eapply IHHfi.
+    + inv Hnu.
+      apply nullable_middle_sym in H0.
+      auto.
+    + destruct hd.
+      * inv Hnu.
+        apply gamma_with_terminal_not_nullable in H0.
+        inv H0.
+      * inv Hfo.
+        inv Hnu.
+        eapply FoLeft; eauto.
+        assert (NT n :: tl = [NT n] ++ tl) by auto.
+        rewrite H1 in H3.
+        rewrite app_assoc in H3.
+        eapply nullable_split in H3.
+        auto.        
+
+  - intros sym gammaPre Hfi Hnu Hfo.
+    eapply IHHfi.
+    + assert (NT x :: tl = [NT x] ++ tl) by auto.
+      rewrite H in Hfi.
+      rewrite app_assoc in Hfi.
+      eauto.
+    + rewrite <- app_assoc.
+      simpl.
+      auto.
+    + rewrite <- app_assoc.
+      simpl.
+      auto.
+
+  - intros Hnu Hfo.
+    inv Hnu.
+    inv H.
+
+  - intros Hnu Hfo.
+    inv Hnu.
+    inv H.
+    assert (Hlk : (@isLookaheadFor g) la (NT x) gamma).
+    { unfold isLookaheadFor.
+      left.
+      auto. }
+    assert (Hlk' : (@isLookaheadFor g) la (NT x) ys).
+    { unfold isLookaheadFor.
+      right.
+      split.
+      { constructor; auto. }
+      { constructor; auto. }}
+    unfold ptComplete in Hcom.
+    apply Hcom in Hlk; apply Hcom in Hlk'.
+    destruct Hlk as [laMap [Hsf Hlf]].
+    destruct Hlk' as [laMap' [Hsf' Hlf']].
+    assert (gamma = ys) by congruence.
+    subst.
+    apply IHHfi.
+    + constructor; auto.
+    + constructor; auto.
+Qed.
+
+Lemma firstGamma_split :
+  forall g la xs ys,
+    (@firstGamma g) la xs
+    -> (@firstGamma g) la (xs ++ ys).
+Proof.
+  induction xs; intros.
+  - inv H.
+  - inv H.
+    + constructor; auto.
+    + eapply FiGammaTl; eauto.
+Qed.
+
+Lemma derives_app :
+  forall g gPre gSuf wPre wSuf fPre fSuf,
+    (@derivesGamma g) gPre wPre fPre
+    -> (@derivesGamma g) gSuf wSuf fSuf
+    -> (@derivesGamma g) (gPre ++ gSuf)
+                         (wPre ++ wSuf)
+                         (appF fPre fSuf).
+Proof.
+  induction gPre; intros; simpl in *.
+  - inv H.
+    auto.
+  - inv H.
+    simpl.
+    rewrite <- app_assoc.
+    constructor.
+    + auto.
+    + apply IHgPre; auto.
+Qed.
+
+Lemma last_case :
+  forall tbl g,
+    isParseTableFor tbl g
+    -> forall sufGamma preGamma x x2 word f f',
+      In (x, preGamma ++ NT x2 :: sufGamma) (productions g)
+      -> (@derivesGamma g) (NT x2 :: sufGamma) word f
+      -> (@derivesGamma g) (NT x2 :: sufGamma) word f'
+      -> f = f'.
+Proof.
+  intros tbl g Htbl.
+  pose proof Htbl as Htbl'.
+  destruct Htbl as [Hmin Hcom].
+  induction sufGamma as [| sym syms].
+  
+Abort.
+
+Lemma derivesSym_det : 
+  forall tbl g,
+    isParseTableFor tbl g
+    -> forall f f' x pre gamma word,
+      In (x, pre ++ gamma) (productions g)
+      -> (@derivesGamma g) gamma word f
+      -> (@derivesGamma g) gamma word f'
+      -> f = f'.
+Proof.
+  intros tbl g Htbl.
+  pose proof Htbl as Htbl'.
+  destruct Htbl as [Hmin Hcom].
+  induction f using forest_mutual_ind with
+      (P := fun tr =>
+              forall tr' sym word,
+                (@derivesSym g) sym word tr
+                -> (@derivesSym g) sym word tr'
+                -> tr = tr').
+  - intros tr' sym word Hder Hder'.
+    inv Hder.
+    + inv Hder'.
+      auto.
+    + inv H.
+
+  - intros tr' sym word Hder Hder'.
+    inv Hder; inv Hder'.
+    inv H; inv H1.
+    assert (gamma = gamma0) by admit.
+    subst.
+    erewrite IHf; eauto.
+    assert (gamma0 = [] ++ gamma0) by auto.
+    rewrite H1 in H.
+    eauto.
+
+  - intros f' x pre gamma word Hin Hder Hder'.
+    inv Hder.
+    inv Hder'.
+    auto.
+
+  - intros f' x pre gamma word Hin Hder Hder'.
+    inv Hder; inv Hder'.
+    destruct tlSyms.
+    + inv H6; inv H4.
+      repeat rewrite app_nil_r in *.
+      subst.
+      erewrite IHf; eauto.
+    + 
+      
+    
+    destruct hdSym as [y | x2].
+    + inv H2; inv H3.
+      inv H1.
+      erewrite IHf0; auto.
+      * assert (T y :: tlSyms = [T y] ++ tlSyms) by auto.
+        rewrite H in Hin.
+        rewrite app_assoc in Hin.
+        eauto.
+      * eauto.
+      * auto.
+    + revert Hin.
+      revert pre.
+      revert 
+      * inv H6.
+        inv H4.
+        repeat rewrite app_nil_r in *.
+        subst.
+        erewrite IHf; eauto.
+      * 
+      
+
+          
+
+      
+(* BEST ATTEMPT SO FAR *)
+
+Lemma derivesSym_det :
+  forall tbl g tr sym word,
+    isParseTableFor tbl g
+    -> (@derivesSym g) sym word tr
+    -> forall tr',
+        (@derivesSym g) sym word tr'
+        -> tr = tr'.
+Proof.
+  intros tbl g tr sym word Htbl Hder.
+  pose proof Htbl as Htbl'.
+  destruct Htbl as [Hmin Hcom].
+  induction Hder using derivesSym_mut_ind with
+      (P := fun x gamma word tr
+                (pf : (@derivesProd g) x gamma word tr) =>
+                 forall tr',
+                   (@derivesProd g) x gamma word tr'
+                   -> tr = tr')
+      (P0 := fun gamma word f
+                 (pf : (@derivesGamma g) gamma word f) =>
+               forall x preGamma f',
+                 In (x, preGamma ++ gamma) (productions g)
+                 -> (@derivesGamma g) gamma word f'
+                 -> f = f').
+  - intros tr' Hderp.
+    inv Hderp.
+    erewrite IHHder; eauto.
+    assert (gamma = [] ++ gamma) by auto.
+    rewrite H1 in i.
+    eauto.
+    
+  - intros x preGamma f' Hin Hderg.
+    inv Hderg.
+    auto.
+
+  - intros x preGamma f' Hin Hderg.
+    pose proof Hderg as Hderg'.
+    inv Hderg.
+    destruct hdSym as [tName | ntName].
+    + inv H2.
+      inv Hder.
+      inv H1.
+      eapply IHHder0 in H4; subst; auto.
+      assert (T tName :: tlSyms = [T tName] ++ tlSyms) by auto.
+      rewrite H in Hin.
+      assert (preGamma ++ [T tName] ++ tlSyms =
+              (preGamma ++ [T tName]) ++ tlSyms).
+      { rewrite app_assoc. auto. }
+      rewrite H0 in Hin.
+      eauto.
+
+    + assert (prefix = prefix0).
+      { (* Maybe I should be doing induction here? *)
+        destruct prefix as [| ptok ptoks] eqn:Hpre;
+          destruct prefix0 as [| ptok' ptoks'] eqn:Hpre';
+          intros; simpl in *.
+        
+        - auto.
+          
+        - (* first / follow *)
+          exfalso.
+          inv Hder.
+          inv H2.
+          assert (Hlk : (@isLookaheadFor g) (LA ptok') (NT ntName) gamma).
+          { unfold isLookaheadFor.
+            right.
+            inv H0.
+            split.
+            { constructor; auto.
+              apply derivesGamma_nil_nullable in H2.
+              auto. }
+            { constructor; auto.
+              eapply FoRight; eauto.
+              apply derivesGamma_cons_firstGamma in d.
+              auto. }}
+          assert (Hlk' : (@isLookaheadFor g) (LA ptok') (NT ntName) gamma0).
+          { unfold isLookaheadFor.
+            left.
+            inv H1.
+            constructor; auto.
+            apply derivesGamma_cons_firstGamma in H2.
+            auto. }
+          unfold ptComplete in Hcom.
+          apply Hcom in Hlk; apply Hcom in Hlk'.
+          destruct Hlk as [laMap [Hsf Hlf]].
+          destruct Hlk' as [laMap' [Hsf' Hlf']].
+          assert (gamma = gamma0) by congruence.
+          subst.
+          inv H0; inv H1.
+          assert ((@firstProd g) (LA ptok') (NT ntName) gamma0).
+          { constructor; auto.
+            apply derivesGamma_cons_firstGamma in H3.
+            auto. }
+          assert ((@nullableProd g) (NT ntName) gamma0).
+          { constructor; auto.
+            apply derivesGamma_nil_nullable in H2.
+            auto. }
+          assert ((@followProd g) (LA ptok') (NT ntName) gamma0).
+          { constructor; auto.
+            econstructor; eauto.
+            apply derivesGamma_cons_firstGamma in d.
+            auto. }
+          eapply no_first_follow_conflicts; eauto.
+          
+        - (* another conflict *)
+          exfalso.
+          inv Hder.
+          inv H2.
+          assert (Hlk : (@isLookaheadFor g) (LA ptok) (NT ntName) gamma0).
+          { unfold isLookaheadFor.
+            right.
+            inv H1.
+            split.
+            { constructor; auto.
+              apply derivesGamma_nil_nullable in H2.
+              auto. }
+            { constructor; auto.
+              eapply FoRight; eauto.
+              apply derivesGamma_cons_firstGamma in H4.
+              auto. }}
+          assert (Hlk' : (@isLookaheadFor g) (LA ptok) (NT ntName) gamma).
+          { unfold isLookaheadFor.
+            left.
+            inv H0.
+            constructor; auto.
+            apply derivesGamma_cons_firstGamma in H2.
+            auto. }
+          unfold ptComplete in Hcom.
+          apply Hcom in Hlk; apply Hcom in Hlk'.
+          destruct Hlk as [laMap [Hsf Hlf]].
+          destruct Hlk' as [laMap' [Hsf' Hlf']].
+          assert (gamma = gamma0) by congruence.
+          subst.
+          inv H0; inv H1.
+          assert ((@firstProd g) (LA ptok) (NT ntName) gamma0).
+          { constructor; auto.
+            apply derivesGamma_cons_firstGamma in H2.
+            auto. }
+          assert ((@nullableProd g) (NT ntName) gamma0).
+          { constructor; auto.
+            apply derivesGamma_nil_nullable in H3.
+            auto. }
+          assert ((@followProd g) (LA ptok) (NT ntName) gamma0).
+          { constructor; auto.
+            econstructor; eauto.
+            apply derivesGamma_cons_firstGamma in H4.
+            auto. }
+          eapply no_first_follow_conflicts; eauto.
+          
+        - inv H1.
+          inv Hder; inv H2.
+          inv H0; inv H1.
+          assert (gamma = gamma0) by admit.
+          subst.
+          admit. }
+
+      assert (suffix0 = suffix) by admit.
+      subst.
+      erewrite IHHder; erewrite IHHder0; eauto.
+      * assert (NT ntName :: tlSyms =
+                [NT ntName] ++ tlSyms) by auto.
+        rewrite H in Hin.
+        rewrite app_assoc in Hin.
+        eauto.
+      * assert (NT ntName :: tlSyms =
+                [NT ntName] ++ tlSyms) by auto.
+        rewrite H in Hin.
+        rewrite app_assoc in Hin.
+        eauto.
+
+  - intros tr' Hder.
+    inv Hder.
+    auto.
+    
+  - intros tr' Hder.
+    inv Hder.
+    inv d; inv H0.
+    pose proof H1 as Hder.
+    pose proof H3 as Hder'.
+    destruct tokens as [| tok toks].
+    + apply derivesGamma_nil_nullable in Hder.
+      apply derivesGamma_nil_nullable in Hder'.
+      assert (Hlk : (@isLookaheadFor g) EOF (NT x) gamma).
+      { unfold isLookaheadFor.
+        right.
+        split.
+        - constructor; auto.
+        - constructor; auto.
+          repeat (econstructor; eauto). }
+      assert (Hlk' : (@isLookaheadFor g) EOF (NT x) gamma0).
+      { unfold isLookaheadFor.
+        right.
+        split.
+        - constructor; auto.
+        - constructor; auto.
+          repeat (econstructor; eauto). }
+      unfold ptComplete in Hcom.
+      apply Hcom in Hlk.
+      apply Hcom in Hlk'.
+      destruct Hlk as [laMap [Hsf Hlf]].
+      destruct Hlk' as [laMap' [Hsf' Hlf']].
+      assert (gamma = gamma0) by congruence.
+      subst.
+      erewrite IHHder; eauto.
+      constructor; auto.
+
+    + apply derivesGamma_cons_firstGamma in Hder.
+      apply derivesGamma_cons_firstGamma in Hder'.
+      assert (Hlk : (@isLookaheadFor g) (LA tok) (NT x) gamma).
+      { unfold isLookaheadFor.
+        left.
+        constructor; auto. }
+      assert (Hlk' : (@isLookaheadFor g) (LA tok) (NT x) gamma0).
+      { unfold isLookaheadFor.
+        left.
+        constructor; auto. }
+      unfold ptComplete in Hcom.
+      apply Hcom in Hlk.
+      apply Hcom in Hlk'.
+      destruct Hlk as [laMap [Hsf Hlf]].
+      destruct Hlk' as [laMap' [Hsf' Hlf']].
+      assert (gamma = gamma0) by congruence.
+      subst.
+      apply IHHder; constructor; auto.
+Admitted.
+    
+
+            
+          (*      
+Lemma last_case :
+  forall tbl g tr f x preGamma ntName tlSyms sufGamma,
+    isParseTableFor tbl g
+    -> (forall tr' sym word,
+           (@derivesSym g) sym word tr
+           -> (@derivesSym g) sym word tr'
+           -> tr = tr')
+    -> (forall f' x preGamma gamma sufGamma word,
+           In (x, preGamma ++ gamma ++ sufGamma)
+              (productions g)
+           -> (@derivesGamma g) gamma word f
+           -> (@derivesGamma g) gamma word f'
+           -> f = f')
+    -> In (x, preGamma ++ (NT ntName :: tlSyms) ++ sufGamma)
+          (productions g)
+    -> forall prefix suffix prefix0 suffix0 hdTree tlTrees,
+        (@derivesSym g) (NT ntName) prefix tr
+        -> (@derivesGamma g) tlSyms suffix f
+        -> (@derivesSym g) (NT ntName) prefix0 hdTree
+        -> (@derivesGamma g) tlSyms suffix0 tlTrees
+        -> prefix0 ++ suffix0 = prefix ++ suffix
+        -> Fcons tr f = Fcons hdTree tlTrees.
+Proof.
+  intros tbl g tr f x preGamma ntName tlSyms sufGamma
+         Htbl IHtr IHf Hin.
+  pose proof Htbl as Htbl'.
+  destruct Htbl as [Hmin Hcom].
+  induction prefix as [| ptok ptoks].
+
+  - intros suffix prefix0 suffix0 hdTree tlTrees
+           Hders Hderg Hders' Hderg' Happ.
+    simpl in *.
+    destruct prefix0 as [| ptok' ptoks']; simpl in *.
+    +  subst.
+       apply IHtr in Hders'; subst; auto.
+       eapply IHf in Hderg'; subst; eauto.
+       assert (NT ntName :: tlSyms = [NT ntName] ++ tlSyms) by auto.
+       rewrite app_comm_cons in Hin.
+       repeat rewrite H in Hin.
+       assert (preGamma ++ [NT ntName] ++ tlSyms =
+               (preGamma ++ [NT ntName]) ++ tlSyms).
+       { rewrite app_assoc; auto. }
+       rewrite app_assoc in Hin.
+       rewrite H0 in Hin.
+       rewrite <- app_assoc in Hin.
+       eauto.
+    + exfalso.
+      inv Hders.
+      inv Hders'.
+      assert (Hlk : (@isLookaheadFor g) (LA ptok') (NT ntName) gamma).
+       { unfold isLookaheadFor.
+         right.
+         inv H0.
+         split.
+         { constructor; auto.
+           apply derivesGamma_nil_nullable in H2.
+           auto. }
+         { constructor; auto.
+           eapply FoRight; eauto.
+           apply derivesGamma_cons_firstGamma in Hderg.
+           apply firstGamma_split.
+           auto. }}
+       assert (Hlk' : (@isLookaheadFor g) (LA ptok') (NT ntName) gamma0).
+       { unfold isLookaheadFor.
+         left.
+         inv H1.
+         constructor; auto.
+         apply derivesGamma_cons_firstGamma in H2.
+         auto. }
+       unfold ptComplete in Hcom.
+       apply Hcom in Hlk; apply Hcom in Hlk'.
+       destruct Hlk as [laMap [Hsf Hlf]].
+       destruct Hlk' as [laMap' [Hsf' Hlf']].
+       assert (gamma = gamma0) by congruence.
+       subst.
+       inv H0; inv H1.
+       assert ((@firstProd g) (LA ptok') (NT ntName) gamma0).
+       { constructor; auto.
+         apply derivesGamma_cons_firstGamma in H3.
+         auto. }
+       assert ((@nullableProd g) (NT ntName) gamma0).
+       { constructor; auto.
+         apply derivesGamma_nil_nullable in H2.
+         auto. }
+       assert ((@followProd g) (LA ptok') (NT ntName) gamma0).
+       { constructor; auto.
+         econstructor; eauto.
+         apply derivesGamma_cons_firstGamma in Hderg.
+         apply firstGamma_split.
+         auto. }
+       eapply no_first_follow_conflicts; eauto.
+    (* Whoa, it worked! *)
+
+  - intros suffix prefix0 suffix0 hdTree tlTrees
+           Hders Hderg Hders' Hderg' Happ.
+    destruct prefix0 as [| ptok' ptoks']; simpl in *.
+    + exfalso.
+      inv Hders'.
+      inv Hders.
+      assert (Hlk : (@isLookaheadFor g) (LA ptok) (NT ntName) gamma).
+      { unfold isLookaheadFor.
+        right.
+        inv H0.
+        split.
+        { constructor; auto.
+          apply derivesGamma_nil_nullable in H2.
+          auto. }
+        { constructor; auto.
+          eapply FoRight; eauto.
+          apply derivesGamma_cons_firstGamma in Hderg'.
+          apply firstGamma_split.
+          auto. }}
+           assert (Hlk' : (@isLookaheadFor g) (LA ptok) (NT ntName) gamma0).
+           { unfold isLookaheadFor.
+             left.
+             inv H1.
+             constructor; auto.
+             apply derivesGamma_cons_firstGamma in H2.
+             auto. }
+           unfold ptComplete in Hcom.
+           apply Hcom in Hlk; apply Hcom in Hlk'.
+           destruct Hlk as [laMap [Hsf Hlf]].
+           destruct Hlk' as [laMap' [Hsf' Hlf']].
+           assert (gamma = gamma0) by congruence.
+           subst.
+           inv H0; inv H1.
+           assert ((@firstProd g) (LA ptok) (NT ntName) gamma0).
+           { constructor; auto.
+             apply derivesGamma_cons_firstGamma in H3.
+             auto. }
+           assert ((@nullableProd g) (NT ntName) gamma0).
+           { constructor; auto.
+             apply derivesGamma_nil_nullable in H2.
+             auto. }
+           assert ((@followProd g) (LA ptok) (NT ntName) gamma0).
+           { constructor; auto.
+             econstructor; eauto.
+             apply derivesGamma_cons_firstGamma in Hderg'.
+             apply firstGamma_split.
+             auto. }
+           eapply no_first_follow_conflicts; eauto.
+    + inv Happ.
+*)      
+
+
+(* putting some padding on both sides of gamma *)
+Lemma derivesSym_det :
+  forall tbl g,
+    isParseTableFor tbl g
+    -> forall tr tr' sym word,
+      (@derivesSym g) sym word tr
+      -> (@derivesSym g) sym word tr'
+      -> tr = tr'.
+Proof.
+  intros tbl g Htbl.
+  pose proof Htbl as Htbl'.
+  destruct Htbl as [Hmin Hcom].
+  induction tr using tree_mutual_ind with
+      (P := fun tr =>
+              forall tr' sym word,
+                (@derivesSym g) sym word tr
+                -> (@derivesSym g) sym word tr'
+                -> tr = tr')
+      (P0 := fun f =>
+               forall f' x preGamma gamma sufGamma word,
+                 In (x, preGamma ++ gamma ++ sufGamma)
+                    (productions g)
+                 -> (@derivesGamma g) gamma word f
+                 -> (@derivesGamma g) gamma word f'
+                 -> f = f').
+
+  - intros tr' sym word Hder Hder'.
+    inv Hder.
+    + inv Hder'.
+      auto.
+    + inv H.
+
+  - intros tr' sym word Hder Hder'.
+    inv Hder; inv Hder'.
+    inv H; inv H1.
+    rename s into x.
+    pose proof H7 as Hder.
+    pose proof H0 as Hder'.
+    destruct word as [| tok toks].
+    + apply derivesGamma_nil_nullable in Hder.
+      apply derivesGamma_nil_nullable in Hder'.
+      assert (Hlk : (@isLookaheadFor g) EOF (NT x) gamma).
+      { unfold isLookaheadFor.
+        right.
+        split.
+        - constructor; auto.
+        - constructor; auto.
+          repeat (econstructor; eauto). }
+      assert (Hlk' : (@isLookaheadFor g) EOF (NT x) gamma0).
+      { unfold isLookaheadFor.
+        right.
+        split.
+        - constructor; auto.
+        - constructor; auto.
+          repeat (econstructor; eauto). }
+      unfold ptComplete in Hcom.
+      apply Hcom in Hlk.
+      apply Hcom in Hlk'.
+      destruct Hlk as [laMap [Hsf Hlf]].
+      destruct Hlk' as [laMap' [Hsf' Hlf']].
+      assert (gamma = gamma0) by congruence.
+      subst.
+      erewrite (IHtr f0); eauto.
+      assert (gamma0 = [] ++ gamma0 ++ []).
+      { rewrite app_nil_r; auto. }
+      rewrite H1 in H.
+      eauto.
+
+    + apply derivesGamma_cons_firstGamma in Hder.
+      apply derivesGamma_cons_firstGamma in Hder'.
+      assert (Hlk : (@isLookaheadFor g) (LA tok) (NT x) gamma).
+      { unfold isLookaheadFor.
+        left.
+        constructor; auto. }
+      assert (Hlk' : (@isLookaheadFor g) (LA tok) (NT x) gamma0).
+      { unfold isLookaheadFor.
+        left.
+        constructor; auto. }
+      unfold ptComplete in Hcom.
+      apply Hcom in Hlk.
+      apply Hcom in Hlk'.
+      destruct Hlk as [laMap [Hsf Hlf]].
+      destruct Hlk' as [laMap' [Hsf' Hlf']].
+      assert (gamma = gamma0) by congruence.
+      subst.
+      erewrite (IHtr f0); eauto.
+      assert (gamma0 = [] ++ gamma0 ++ []).
+      { rewrite app_nil_r; auto. }
+      rewrite H1 in H.
+      eauto.
+
+  - intros f' x preGamma gamma sufGamma word Hin Hder Hder'.
+    inv Hder.
+    inv Hder'.
+    auto.
+
+  - intros f' x preGamma gamma sufGamma word Hin Hder Hder'.
+    inv Hder.
+    inv Hder'.
+    destruct hdSym as [tName | ntName].
+    + inv H2.
+      inv H3.
+      inv H1.
+      eapply IHtr0 in H6; subst; auto.
+      assert (T tName :: tlSyms = [T tName] ++ tlSyms) by auto.
+      rewrite H in Hin.
+      assert (preGamma ++ [T tName] ++ tlSyms =
+              (preGamma ++ [T tName]) ++ tlSyms).
+      { rewrite app_assoc. auto. }
+      rewrite app_assoc in Hin.
+      rewrite H0 in Hin.
+      rewrite <- app_assoc in Hin.
+      eauto.
+    + destruct prefix as [| ptok ptoks].
+      * simpl in *.
+        subst.
+        destruct prefix0 as [| ptok' ptoks']; simpl in *.
+        -- apply IHtr in H2; subst; auto.
+           eapply IHtr0 in H6; subst; eauto.
+           assert (NT ntName :: tlSyms = [NT ntName] ++ tlSyms) by auto.
+           rewrite app_comm_cons in Hin.
+           repeat rewrite H in Hin.
+           assert (preGamma ++ [NT ntName] ++ tlSyms =
+                   (preGamma ++ [NT ntName]) ++ tlSyms).
+           { rewrite app_assoc; auto. }
+           rewrite app_assoc in Hin.
+           rewrite H0 in Hin.
+           rewrite <- app_assoc in Hin.
+           eauto.
+        -- exfalso.
+           inv H3.
+           inv H2.
+           assert (Hlk : (@isLookaheadFor g) (LA ptok') (NT ntName) gamma).
+           { unfold isLookaheadFor.
+             right.
+             inv H0.
+             split.
+             { constructor; auto.
+               apply derivesGamma_nil_nullable in H2.
+               auto. }
+             { constructor; auto.
+               eapply FoRight; eauto.
+               apply derivesGamma_cons_firstGamma in H4.
+               apply firstGamma_split.
+               auto. }}
+           assert (Hlk' : (@isLookaheadFor g) (LA ptok') (NT ntName) gamma0).
+           { unfold isLookaheadFor.
+             left.
+             inv H1.
+             constructor; auto.
+             apply derivesGamma_cons_firstGamma in H2.
+             auto. }
+           unfold ptComplete in Hcom.
+           apply Hcom in Hlk; apply Hcom in Hlk'.
+           destruct Hlk as [laMap [Hsf Hlf]].
+           destruct Hlk' as [laMap' [Hsf' Hlf']].
+           assert (gamma = gamma0) by congruence.
+           subst.
+           inv H0; inv H1.
+           assert ((@firstProd g) (LA ptok') (NT ntName) gamma0).
+           { constructor; auto.
+             apply derivesGamma_cons_firstGamma in H3.
+             auto. }
+           assert ((@nullableProd g) (NT ntName) gamma0).
+           { constructor; auto.
+             apply derivesGamma_nil_nullable in H2.
+             auto. }
+           assert ((@followProd g) (LA ptok') (NT ntName) gamma0).
+           { constructor; auto.
+             econstructor; eauto.
+             apply derivesGamma_cons_firstGamma in H4.
+             apply firstGamma_split.
+             auto. }
+           eapply no_first_follow_conflicts; eauto.
+           (* Whoa, it worked! *)
+
+      * destruct prefix0 as [| ptok' ptoks']; simpl in *.
+        -- exfalso.
+           inv H2.
+           inv H3.
+           assert (Hlk : (@isLookaheadFor g) (LA ptok) (NT ntName) gamma).
+           { unfold isLookaheadFor.
+             right.
+             inv H0.
+             split.
+             { constructor; auto.
+               apply derivesGamma_nil_nullable in H2.
+               auto. }
+             { constructor; auto.
+               eapply FoRight; eauto.
+               apply derivesGamma_cons_firstGamma in H6.
+               apply firstGamma_split.
+               auto. }}
+           assert (Hlk' : (@isLookaheadFor g) (LA ptok) (NT ntName) gamma0).
+           { unfold isLookaheadFor.
+             left.
+             inv H1.
+             constructor; auto.
+             apply derivesGamma_cons_firstGamma in H2.
+             auto. }
+           unfold ptComplete in Hcom.
+           apply Hcom in Hlk; apply Hcom in Hlk'.
+           destruct Hlk as [laMap [Hsf Hlf]].
+           destruct Hlk' as [laMap' [Hsf' Hlf']].
+           assert (gamma = gamma0) by congruence.
+           subst.
+           inv H0; inv H1.
+           assert ((@firstProd g) (LA ptok) (NT ntName) gamma0).
+           { constructor; auto.
+             apply derivesGamma_cons_firstGamma in H3.
+             auto. }
+           assert ((@nullableProd g) (NT ntName) gamma0).
+           { constructor; auto.
+             apply derivesGamma_nil_nullable in H2.
+             auto. }
+           assert ((@followProd g) (LA ptok) (NT ntName) gamma0).
+           { constructor; auto.
+             econstructor; eauto.
+             apply derivesGamma_cons_firstGamma in H6.
+             apply firstGamma_split.
+             auto. }
+           eapply no_first_follow_conflicts; eauto.
+
+        -- inv H1.
+           
+
+Lemma derivesSym_det :
+  forall tbl g,
+    isParseTableFor tbl g
+    -> forall tr tr' sym word,
+      (@derivesSym g) sym word tr
+      -> (@derivesSym g) sym word tr'
+      -> tr = tr'.
+Proof.
+  intros tbl g Htbl.
+  pose proof Htbl as Htbl'.
+  destruct Htbl as [Hmin Hcom].
+  induction tr using tree_mutual_ind with
+      (P := fun tr =>
+              forall tr' sym word,
+                (@derivesSym g) sym word tr
+                -> (@derivesSym g) sym word tr'
+                -> tr = tr')
+      (P0 := fun sufF =>
+               forall sufF' x preGamma sufGamma sufWord,
+                 In (x, preGamma ++ sufGamma) (productions g)
+                 -> (@derivesGamma g) sufGamma sufWord
+                                      sufF
+                 -> (@derivesGamma g) sufGamma sufWord
+                                      sufF'
+                 -> sufF = sufF').
+
+  - intros tr' sym word Hder Hder'.
+    inv Hder.
+    + inv Hder'.
+      auto.
+    + inv H.
+
+  - intros tr' sym word Hder Hder'.
+    inv Hder; inv Hder'.
+    inv H; inv H1.
+    rename s into x.
+    pose proof H7 as Hder.
+    pose proof H0 as Hder'.
+    destruct word as [| tok toks].
+    + apply derivesGamma_nil_nullable in Hder.
+      apply derivesGamma_nil_nullable in Hder'.
+      assert (Hlk : (@isLookaheadFor g) EOF (NT x) gamma).
+      { unfold isLookaheadFor.
+        right.
+        split.
+        - constructor; auto.
+        - constructor; auto.
+          repeat (econstructor; eauto). }
+      assert (Hlk' : (@isLookaheadFor g) EOF (NT x) gamma0).
+      { unfold isLookaheadFor.
+        right.
+        split.
+        - constructor; auto.
+        - constructor; auto.
+          repeat (econstructor; eauto). }
+      unfold ptComplete in Hcom.
+      apply Hcom in Hlk.
+      apply Hcom in Hlk'.
+      destruct Hlk as [laMap [Hsf Hlf]].
+      destruct Hlk' as [laMap' [Hsf' Hlf']].
+      assert (gamma = gamma0) by congruence.
+      subst.
+      erewrite (IHtr f0); eauto.
+      assert (gamma0 = [] ++ gamma0).
+      { rewrite app_nil_l. auto. }
+      rewrite H1 in H.
+      eauto.
+
+    + apply derivesGamma_cons_firstGamma in Hder.
+      apply derivesGamma_cons_firstGamma in Hder'.
+      assert (Hlk : (@isLookaheadFor g) (LA tok) (NT x) gamma).
+      { unfold isLookaheadFor.
+        left.
+        constructor; auto. }
+      assert (Hlk' : (@isLookaheadFor g) (LA tok) (NT x) gamma0).
+      { unfold isLookaheadFor.
+        left.
+        constructor; auto. }
+      unfold ptComplete in Hcom.
+      apply Hcom in Hlk.
+      apply Hcom in Hlk'.
+      destruct Hlk as [laMap [Hsf Hlf]].
+      destruct Hlk' as [laMap' [Hsf' Hlf']].
+      assert (gamma = gamma0) by congruence.
+      subst.
+      erewrite (IHtr f0); eauto.
+      assert (gamma0 = [] ++ gamma0) by auto.
+      rewrite H1 in H.
+      eauto.
+
+  - intros preF' x preGamma sufGamma preWord Hin Hder Hder'.
+    inv Hder.
+    inv Hder'.
+    auto.
+
+  - intros sufF' x preGamma sufGamma sufWord Hin Hder Hder'.
+    inv Hder.
+    inv Hder'.
+    destruct hdSym as [tName | ntName].
+    + inv H2.
+      inv H3.
+      inv H1.
+      eapply IHtr0 in H6; subst; eauto.
+      assert (T tName :: tlSyms = [T tName] ++ tlSyms) by auto.
+      rewrite H in Hin.
+      rewrite app_assoc in Hin.
+      eauto.
+    + destruct prefix as [| ptok ptoks].
+      * simpl in *.
+        subst.
+        destruct prefix0 as [| ptok' ptoks']; simpl in *.
+        -- apply IHtr in H2; subst; auto.
+           eapply IHtr0 in H6; subst; eauto.
+           assert (NT ntName :: tlSyms = [NT ntName] ++ tlSyms) by auto.
+      rewrite H in Hin.
+      rewrite app_assoc in Hin.
+      eauto.
+        -- exfalso.
+           pose proof H3 as Hder.
+           inv H3.
+           inv H2.
+           assert (Hlk : (@isLookaheadFor g) (LA ptok') (NT ntName) gamma).
+           { unfold isLookaheadFor.
+             right.
+             inv H0.
+             split.
+             { constructor; auto.
+               apply derivesGamma_nil_nullable in H2.
+               auto. }
+             { constructor; auto.
+               eapply FoRight; eauto.
+               apply derivesGamma_cons_firstGamma in H4.
+               auto. }}
+           assert (Hlk' : (@isLookaheadFor g) (LA ptok') (NT ntName) gamma0).
+           { unfold isLookaheadFor.
+             left.
+             inv H1.
+             constructor; auto.
+             apply derivesGamma_cons_firstGamma in H2.
+             auto. }
+           unfold ptComplete in Hcom.
+           apply Hcom in Hlk; apply Hcom in Hlk'.
+           destruct Hlk as [laMap [Hsf Hlf]].
+           destruct Hlk' as [laMap' [Hsf' Hlf']].
+           assert (gamma = gamma0) by congruence.
+           subst.
+           inv H0; inv H1.
+           assert ((@firstProd g) (LA ptok') (NT ntName) gamma0).
+           { constructor; auto.
+             apply derivesGamma_cons_firstGamma in H3.
+             auto. }
+           assert ((@nullableProd g) (NT ntName) gamma0).
+           { constructor; auto.
+             apply derivesGamma_nil_nullable in H2.
+             auto. }
+           assert ((@followProd g) (LA ptok') (NT ntName) gamma0).
+           { constructor; auto.
+             econstructor; eauto.
+             apply derivesGamma_cons_firstGamma in H4.
+             auto. }
+           eapply no_first_follow_conflicts; eauto.
+           (* Whoa, it worked! *)
+
+      * destruct prefix0 as [| ptok' ptoks']; simpl in *.
+        -- exfalso.
+           inv H2.
+           inv H3.
+           assert (Hlk : (@isLookaheadFor g) (LA ptok) (NT ntName) gamma).
+           { unfold isLookaheadFor.
+             right.
+             inv H0.
+             split.
+             { constructor; auto.
+               apply derivesGamma_nil_nullable in H2.
+               auto. }
+             { constructor; auto.
+               eapply FoRight; eauto.
+               apply derivesGamma_cons_firstGamma in H6.
+               auto. }}
+           assert (Hlk' : (@isLookaheadFor g) (LA ptok) (NT ntName) gamma0).
+           { unfold isLookaheadFor.
+             left.
+             inv H1.
+             constructor; auto.
+             apply derivesGamma_cons_firstGamma in H2.
+             auto. }
+           unfold ptComplete in Hcom.
+           apply Hcom in Hlk; apply Hcom in Hlk'.
+           destruct Hlk as [laMap [Hsf Hlf]].
+           destruct Hlk' as [laMap' [Hsf' Hlf']].
+           assert (gamma = gamma0) by congruence.
+           subst.
+           inv H0; inv H1.
+           assert ((@firstProd g) (LA ptok) (NT ntName) gamma0).
+           { constructor; auto.
+             apply derivesGamma_cons_firstGamma in H3.
+             auto. }
+           assert ((@nullableProd g) (NT ntName) gamma0).
+           { constructor; auto.
+             apply derivesGamma_nil_nullable in H2.
+             auto. }
+           assert ((@followProd g) (LA ptok) (NT ntName) gamma0).
+           { constructor; auto.
+             econstructor; eauto.
+             apply derivesGamma_cons_firstGamma in H6.
+             auto. }
+           eapply no_first_follow_conflicts; eauto.
+
+        -- inv H1.
+           
+              
+           
+        
+        
+               
+
+
+
+
+
+
+
+
+              
+             assert (Hder : (@derivesGamma g) (NT ntName :: tlSyms)
+                                            (ptok' :: ptoks')
+                                            (Fcons tr f)).
+           { assert (ptok' :: ptoks' =
+                     [] ++ (ptok' :: ptoks'))
+               by auto.
+             rewrite H.
+             econstructor; eauto. }
+           assert (Hder' : (@derivesGamma g) (NT ntName :: tlSyms)
+                                             (ptok' :: ptoks')
+                                             (Fcons hdTree tlTrees)).
+           { assert (ptok' :: ptoks' =
+                     ptok' :: ptoks' ++ []).
+             { rewrite app_nil_r. auto. }
+             rewrite H.
+             rewrite app_comm_cons.
+             econstructor; eauto. }
+           
+Abort.      
+      
+
+Fixpoint inF tr f :=
+  match f with
+  | Fnil => False
+  | Fcons tr' f' => tr = tr' \/ inF tr f'
+  end.
+
+Lemma derivesSym_det :
+  forall tbl g,
+    isParseTableFor tbl g
+    -> forall tr tr' sym word,
+      (@derivesSym g) sym word tr
+      -> (@derivesSym g) sym word tr'
+      -> tr = tr'.
+Proof.
+  intros tbl g Htbl.
+  destruct Htbl as [Hmin Hcom].
+  induction tr using tree_nested_ind with
+      (Q := fun preF =>
+              forall preF' x preGamma sufGamma
+                     preWord sufWord
+                     sufF,
+                In (x, preGamma ++ sufGamma) (productions g)
+                -> (@derivesGamma g) preGamma preWord preF
+                -> (@derivesGamma g) preGamma preWord preF'
+                -> (@derivesGamma g) sufGamma sufWord sufF
+                -> preF = preF').
+
+Fixpoint inF tr f :=
+  match f with
+  | Fnil => False
+  | Fcons tr' f' => tr = tr' \/ inF tr f'
+  end.
+
+Lemma derivesSym_det :
+  forall tbl g,
+    isParseTableFor tbl g
+    -> forall tr tr' sym word,
+      (@derivesSym g) sym word tr
+      -> (@derivesSym g) sym word tr'
+      -> tr = tr'.
+Proof.
+  intros tbl g Htbl.
+  destruct Htbl as [Hmin Hcom].
+  induction tr using tree_mutual_ind with
+      (P := fun tr =>
+              forall tr' sym word,
+                (@derivesSym g) sym word tr
+                -> (@derivesSym g) sym word tr'
+                -> tr = tr')
+      (P0 := fun f =>
+               forall tr tr' sym,
+                 
+                      
+                 In (x, gamma) (productions g)
+                 -> (@derivesGamma g) gamma word (appF fPre f)
+                 -> (@derivesGamma g) gamma word (appF fPre f')
+                 -> f = f').
+
+
+
+Lemma derivesSym_det :
+  forall tbl g,
+    isParseTableFor tbl g
+    -> forall tr tr' sym word,
+      (@derivesSym g) sym word tr
+      -> (@derivesSym g) sym word tr'
+      -> tr = tr'.
+Proof.
+  intros tbl g Htbl.
+  destruct Htbl as [Hmin Hcom].
+  induction tr using tree_mutual_ind with
+      (P := fun tr =>
+              forall tr' sym word,
+                (@derivesSym g) sym word tr
+                -> (@derivesSym g) sym word tr'
+                -> tr = tr')
+      (P0 := fun sufF =>
+               forall sufF' preF x gamma word,
+                 In (x, gamma) (productions g)
+                 -> (@derivesGamma g) gamma word
+                                      (appF preF sufF)
+                 -> (@derivesGamma g) gamma word
+                                      (appF preF sufF')
+                 -> sufF = sufF').
+
+  - intros tr' sym word Hder Hder'.
+    inv Hder.
+    + inv Hder'.
+      auto.
+    + inv H.
+
+  - intros tr' sym word Hder Hder'.
+    inv Hder; inv Hder'.
+    inv H; inv H1.
+    rename s into x.
+    pose proof H7 as Hder.
+    pose proof H0 as Hder'.
+    destruct word as [| tok toks].
+    + apply derivesGamma_nil_nullable in Hder.
+      apply derivesGamma_nil_nullable in Hder'.
+      assert (Hlk : (@isLookaheadFor g) EOF x gamma).
+      { unfold isLookaheadFor.
+        right.
+        split.
+        - constructor; auto.
+        - constructor; auto.
+          repeat (econstructor; eauto). }
+      assert (Hlk' : (@isLookaheadFor g) EOF x gamma0).
+      { unfold isLookaheadFor.
+        right.
+        split.
+        - constructor; auto.
+        - constructor; auto.
+          repeat (econstructor; eauto). }
+      unfold ptComplete in Hcom.
+      apply Hcom in Hlk.
+      apply Hcom in Hlk'.
+      destruct Hlk as [laMap [Hsf Hlf]].
+      destruct Hlk' as [laMap' [Hsf' Hlf']].
+      assert (gamma = gamma0) by congruence.
+      subst.
+      erewrite (IHtr f0); eauto.
+      * assert (f = appF Fnil f) by auto.
+        rewrite H1 in H7.
+        eauto. 
+      * simpl. auto.
+    + apply derivesGamma_cons_firstGamma in Hder.
+      apply derivesGamma_cons_firstGamma in Hder'.
+      assert (Hlk : (@isLookaheadFor g) (LA tok) x gamma).
+      { unfold isLookaheadFor.
+        left.
+        constructor; auto. }
+      assert (Hlk' : (@isLookaheadFor g) (LA tok) x gamma0).
+      { unfold isLookaheadFor.
+        left.
+        constructor; auto. }
+      unfold ptComplete in Hcom.
+      apply Hcom in Hlk.
+      apply Hcom in Hlk'.
+      destruct Hlk as [laMap [Hsf Hlf]].
+      destruct Hlk' as [laMap' [Hsf' Hlf']].
+      assert (gamma = gamma0) by congruence.
+      subst.
+      erewrite (IHtr f0); eauto.
+      * assert (f = appF Fnil f) by auto.
+        rewrite H1 in H7.
+        eauto. 
+      * simpl. auto.
+
+  - intros sufF' preF x gamma word
+           Hin Hder Hder'.
+    rewrite appF_nil_r in Hder.
+    destruct sufF'.
+    + auto.
+    + apply forest_length in Hder.
+      apply forest_length in Hder'.
+      rewrite Hder in Hder'.
+      apply lengths_contra in Hder'.
+      inv Hder'.
+
+  - intros sufF' preF x gamma word Hin Hder Hder'.
+    assert (appF preF (Fcons tr f) =
+            appF preF (appF (Fcons tr Fnil) f)) by auto.
+    rewrite H in Hder.
+    clear H.
+    rewrite app
+    inv Hder.
+    + apply appF_Fcons_not_Fnil in H2.
+      inv H2.
+    + inv Hder'.
+      destruct hdSym as [tName | ntName].
+      * inv H0.
+        inv H6.
+        inv H4.
+        
+        destruct f
+        assert (appF preF (Fcons tr f) =
+                appF preF (appF (Fcons tr Fnil) f)).
+        { auto. }
+        rewrite H0 in H.
+        
+    
+    
+
+    
+  - intros sufF' x preGamma sufGamma preWord sufWord preF
+           Hin Hderp Hders Hders'.
+    simpl in *.
+    inv Hders.
+    inv Hders'.
+    destruct hdSym as [tName | ntName].
+    + inv H3.
+      inv H2.
+      inv H1.
+      eapply IHtr0 in H6; subst; auto.
+      * assert (T tName :: tlSyms = [T tName] ++ tlSyms)
+          by auto.
+        rewrite H in Hin.
+        rewrite app_assoc in Hin.
+        eauto.
+      * eapply derives_app.
+        -- eauto.
+        -- repeat econstructor.
+    + destruct prefix as [| ptok ptoks]; simpl in *.
+      * destruct prefix0 as [| ptok' ptoks']; simpl in *.
+        -- subst.
+           erewrite IHtr; eauto.
+           erewrite IHtr0; auto.
+           ++ assert (NT ntName :: tlSyms =
+                      [NT ntName] ++ tlSyms) by auto.
+              rewrite H in Hin.
+              rewrite app_assoc in Hin.
+              eauto.
+           ++ eapply derives_app.
+              ** eauto.
+              ** econstructor.
+                 eauto.
+                 econstructor.
+           ++ eauto.
+           ++ auto.
+        -- destruct suffix as [| stok stoks].
+           ++ inv H1.
+           ++ inv H1.
+
+Lemma derivesSym_det :
+  forall tbl g,
+    isParseTableFor tbl g
+    -> forall tr tr' sym word,
+      (@derivesSym g) sym word tr
+      -> (@derivesSym g) sym word tr'
+      -> tr = tr'.
+Proof.
+  intros tbl g Htbl.
+  destruct Htbl as [Hmin Hcom].
+  induction tr using tree_mutual_ind with
+      (P := fun tr =>
+              forall tr' sym word,
+                (@derivesSym g) sym word tr
+                -> (@derivesSym g) sym word tr'
+                -> tr = tr')
+      (P0 := fun sufF =>
+               forall sufF' x preGamma sufGamma
+                      preWord sufWord preF,
+                 In (x, gamma) (productions g)
+                 -> (@derivesGamma g) preGamma preWord preF
+                 -> (@derivesGamma g) sufGamma sufWord sufF
+                 -> (@derivesGamma g) sufGamma sufWord sufF'
+                 -> sufF = sufF').
+
+  - intros tr' sym word Hder Hder'.
+    inv Hder.
+    + inv Hder'.
+      auto.
+    + inv H.
+
+  - intros tr' sym word Hder Hder'.
+    inv Hder; inv Hder'.
+    inv H; inv H1.
+    rename s into x.
+    pose proof H7 as Hder.
+    pose proof H0 as Hder'.
+    destruct word as [| tok toks].
+    + apply derivesGamma_nil_nullable in Hder.
+      apply derivesGamma_nil_nullable in Hder'.
+      assert (Hlk : (@isLookaheadFor g) EOF x gamma).
+      { unfold isLookaheadFor.
+        right.
+        split.
+        - constructor; auto.
+        - constructor; auto.
+          repeat (econstructor; eauto). }
+      assert (Hlk' : (@isLookaheadFor g) EOF x gamma0).
+      { unfold isLookaheadFor.
+        right.
+        split.
+        - constructor; auto.
+        - constructor; auto.
+          repeat (econstructor; eauto). }
+      unfold ptComplete in Hcom.
+      apply Hcom in Hlk.
+      apply Hcom in Hlk'.
+      destruct Hlk as [laMap [Hsf Hlf]].
+      destruct Hlk' as [laMap' [Hsf' Hlf']].
+      assert (gamma = gamma0) by congruence.
+      subst.
+      erewrite (IHtr f0); auto.
+      * assert (gamma0 = nil ++ gamma0) by auto.
+        rewrite H1 in H.
+        eauto.
+      * econstructor. 
+      * eauto.
+      * eauto. 
+    + apply derivesGamma_cons_firstGamma in Hder.
+      apply derivesGamma_cons_firstGamma in Hder'.
+      assert (Hlk : (@isLookaheadFor g) (LA tok) x gamma).
+      { unfold isLookaheadFor.
+        left.
+        constructor; auto. }
+      assert (Hlk' : (@isLookaheadFor g) (LA tok) x gamma0).
+      { unfold isLookaheadFor.
+        left.
+        constructor; auto. }
+      unfold ptComplete in Hcom.
+      apply Hcom in Hlk.
+      apply Hcom in Hlk'.
+      destruct Hlk as [laMap [Hsf Hlf]].
+      destruct Hlk' as [laMap' [Hsf' Hlf']].
+      assert (gamma = gamma0) by congruence.
+      subst.
+      erewrite (IHtr f0); auto.
+      * assert (gamma0 = nil ++ gamma0) by auto.
+        rewrite H1 in H.
+        eauto.
+      * econstructor. 
+      * eauto.
+      * auto.
+
+  - intros sufF' x preGamma sufGamma preWord sufWord preF
+           Hin Hderp Hders Hders'.
+    inv Hders.
+    inv Hders'.
+    auto.
+
+  - intros sufF' x preGamma sufGamma preWord sufWord preF
+           Hin Hderp Hders Hders'.
+    simpl in *.
+    inv Hders.
+    inv Hders'.
+    destruct hdSym as [tName | ntName].
+    + inv H3.
+      inv H2.
+      inv H1.
+      eapply IHtr0 in H6; subst; auto.
+      * assert (T tName :: tlSyms = [T tName] ++ tlSyms)
+          by auto.
+        rewrite H in Hin.
+        rewrite app_assoc in Hin.
+        eauto.
+      * eapply derives_app.
+        -- eauto.
+        -- repeat econstructor.
+    + destruct prefix as [| ptok ptoks]; simpl in *.
+      * destruct prefix0 as [| ptok' ptoks']; simpl in *.
+        -- subst.
+           erewrite IHtr; eauto.
+           erewrite IHtr0; auto.
+           ++ assert (NT ntName :: tlSyms =
+                      [NT ntName] ++ tlSyms) by auto.
+              rewrite H in Hin.
+              rewrite app_assoc in Hin.
+              eauto.
+           ++ eapply derives_app.
+              ** eauto.
+              ** econstructor.
+                 eauto.
+                 econstructor.
+           ++ eauto.
+           ++ auto.
+        -- destruct suffix as [| stok stoks].
+           ++ inv H1.
+           ++ inv H1.
+              
+    
+
+              
+(* try induction on derives *)
+Lemma derivesSym_det :
+  forall tbl g sym word tr,
+    isParseTableFor tbl g
+    -> (@derivesSym g) sym word tr
+    -> forall tr',
+        (@derivesSym g) sym word tr'
+        -> tr = tr'.
+Proof.
+  intros tbl g sym word tr Htbl Hder.
+  induction Hder using derivesSym_mutual_ind with
+      (P := fun x gamma word tr
+                (pf : (@derivesProd g) x gamma word tr) =>
+              forall tr',
+                (@derivesProd g) x gamma word tr'
+                -> tr = tr')
+      (P0 := fun sym word tr
+                 (pf : (@derivesSym g) sym word tr) =>
+               forall tr',
+                 (@derivesSym g) sym word tr'
+                 -> tr = tr')
+      (P1 := fun gSuf wSuf fSuf
+                 (pf : (@derivesGamma g) gSuf wSuf fSuf) =>
+               forall x gPre wPre fPre fSuf',
+                 In (x, gPre ++ gSuf) (productions g)
+                 -> (@derivesGamma g) (gPre ++ gSuf)
+                                      (wPre ++ wSuf)
+                                      (appF fPre fSuf)
+                 -> (@derivesGamma g) (gPre ++ gSuf)
+                                      (wPre ++ wSuf)
+                                      (appF fPre fSuf')
+                 -> fSuf = fSuf').
+      
+  - intros tr' Hder.
+    inv Hder.
+    erewrite IHHder; auto.
+    + assert (gamma = [] ++ gamma) by auto.
+      rewrite H1 in i.
+      eauto.
+    + simpl.
+      assert (tokens = [] ++ tokens) by auto.
+      rewrite H1 in d.
+      assert (f = appF Fnil f) by auto.
+      rewrite H2 in d.
+      eauto.
+    + simpl.
+      auto.
+
+  - intros tr' Hder.
+    inv Hder.
+    auto.
+
+  - intros tr' Hder.
+    inv Hder.
+    apply IHHder; clear IHHder.
+    (* prove gamma = gamma0 *)
+    destruct Htbl as [Hmin Hcom].
+    inv d; inv H0.
+    pose proof H1 as Hder.
+    pose proof H3 as Hder'.
+    destruct tokens as [| tok toks].
+    + constructor; auto.
+      apply derivesGamma_nil_nullable in Hder.
+      apply derivesGamma_nil_nullable in Hder'.
+      assert (Hlk : (@isLookaheadFor g) EOF x gamma).
+      { unfold isLookaheadFor.
+        right.
+        split.
+        - constructor; auto.
+        - constructor; auto.
+          repeat (econstructor; eauto). }
+      assert (Hlk' : (@isLookaheadFor g) EOF x gamma0).
+      { unfold isLookaheadFor.
+        right.
+        split.
+        - constructor; auto.
+        - constructor; auto.
+          repeat (econstructor; eauto). }
+      unfold ptComplete in Hcom.
+      apply Hcom in Hlk.
+      apply Hcom in Hlk'.
+      destruct Hlk as [laMap [Hsf Hlf]].
+      destruct Hlk' as [laMap' [Hsf' Hlf']].
+      assert (gamma = gamma0) by congruence.
+      subst.
+      auto.
+
+    + apply derivesGamma_cons_firstGamma in Hder.
+      apply derivesGamma_cons_firstGamma in Hder'.
+      assert (Hlk : (@isLookaheadFor g) (LA tok) x gamma).
+      { unfold isLookaheadFor.
+        left.
+        constructor; auto. }
+      assert (Hlk' : (@isLookaheadFor g) (LA tok) x gamma0).
+      { unfold isLookaheadFor.
+        left.
+        constructor; auto. }
+      unfold ptComplete in Hcom.
+      apply Hcom in Hlk.
+      apply Hcom in Hlk'.
+      destruct Hlk as [laMap [Hsf Hlf]].
+      destruct Hlk' as [laMap' [Hsf' Hlf']].
+      assert (gamma = gamma0) by congruence.
+      subst.
+      constructor; auto.
+
+  - intros x gPre wPre fPre fSuf' Hin Hder Hder'.
+    repeat rewrite app_nil_r in *.
+    rewrite appF_nil_r in Hder.
+    destruct fSuf'.
+    + auto.
+    + apply forest_length in Hder.
+      apply forest_length in Hder'.
+      rewrite Hder in Hder'.
+      apply lengths_contra in Hder'.
+      inv Hder'.
+
+  - intros x gPre xPre fPre fSuf' Hin Hder1 Hder2.
+    
+     
+      
+    
+
+
+Lemma derivesSym_det :
+  forall tbl g,
+    isParseTableFor tbl g
+    -> forall tr tr' sym tokens,
+      (@derivesSym g) sym tokens tr
+      -> (@derivesSym g) sym tokens tr'
+      -> tr = tr'.
+Proof.
+  intros tbl g Htbl.
+  induction tr using tree_mutual_ind with
+      (P := fun tr =>
+              forall tr' sym tokens,
+                (@derivesSym g) sym tokens tr
+                -> (@derivesSym g) sym tokens tr'
+                -> tr = tr')
+      (P0 := fun fSuf =>
+               forall fSuf' fPre x gPre gSuf wPre wSuf,
+                 In (x, gPre ++ gSuf) (productions g)
+                 -> (@derivesGamma g) gPre wPre fPre
+                 -> (@derivesGamma g) gSuf wSuf fSuf
+                 -> (@derivesGamma g) gSuf wSuf fSuf'
+                 -> fSuf = fSuf').
+
+  - intros tr' sym tokens Hder Hder'.
+    inv Hder.
+    + inv Hder'.
+      auto.
+    + inv H.
+
+  - intros tr' sym tokens Hder Hder'.
+    inv Hder; inv Hder'.
+    inv H; inv H1.
+    pose proof H7 as Hder.
+    pose proof H0 as Hder'.
+    rename s into x.
+    destruct Htbl as [Hmin Hcom].
+    destruct tokens as [| tok toks].
+    + apply derivesGamma_nil_nullable in Hder.
+      apply derivesGamma_nil_nullable in Hder'.
+      assert (Hlk : (@isLookaheadFor g) EOF x gamma).
+      { unfold isLookaheadFor.
+        right.
+        split.
+        - constructor; auto.
+        - constructor; auto.
+          repeat (econstructor; eauto). }
+      assert (Hlk' : (@isLookaheadFor g) EOF x gamma0).
+      { unfold isLookaheadFor.
+        right.
+        split.
+        - constructor; auto.
+        - constructor; auto.
+          repeat (econstructor; eauto). }
+      unfold ptComplete in Hcom.
+      apply Hcom in Hlk.
+      apply Hcom in Hlk'.
+      destruct Hlk as [laMap [Hsf Hlf]].
+      destruct Hlk' as [laMap' [Hsf' Hlf']].
+      assert (gamma = gamma0) by congruence.
+      subst.
+      erewrite (IHtr f0); auto.
+      * assert (nil ++ gamma0 = gamma0) by apply app_nil_l.
+        rewrite <- H1 in H.
+        eauto.
+      * econstructor.
+      * eauto.
+      * auto.
+    + apply derivesGamma_cons_firstGamma in Hder.
+      apply derivesGamma_cons_firstGamma in Hder'.
+      assert (Hlk : (@isLookaheadFor g) (LA tok) x gamma).
+      { unfold isLookaheadFor.
+        left.
+        constructor; auto. }
+      assert (Hlk' : (@isLookaheadFor g) (LA tok) x gamma0).
+      { unfold isLookaheadFor.
+        left.
+        constructor; auto. }
+      unfold ptComplete in Hcom.
+      apply Hcom in Hlk.
+      apply Hcom in Hlk'.
+      destruct Hlk as [laMap [Hsf Hlf]].
+      destruct Hlk' as [laMap' [Hsf' Hlf']].
+      assert (gamma = gamma0) by congruence.
+      subst.
+      erewrite (IHtr f0); auto.
+      * assert (nil ++ gamma0 = gamma0) by apply app_nil_l.
+        rewrite <- H1 in H.
+        eauto.
+      * econstructor.
+      * eauto.
+      * auto.
+
+  - intros fSuf' fPre x gPre gSuf wPre wSuf
+           Hin HderPre HderSuf HderSuf'.
+    inv HderSuf.
+    inv HderSuf'.
+    auto.
+
+  - intros fSuf' fPre x gPre gSuf wPre wSuf
+           Hin Hderp Hders Hders'.
+    inv Hders; inv Hders'.
+    destruct hdSym as [tName | ntName].
+    + inv H3; inv H2.
+      inv H1.
+      eapply IHtr0 in H6; auto.
+      * subst.
+        auto.
+      * assert (T tName :: tlSyms = [T tName] ++ tlSyms)
+          by auto.
+        rewrite H in Hin.
+        rewrite app_assoc in Hin.
+        eauto.
+      * eapply derives_app; eauto; repeat constructor.
+    + destruct prefix as [| ptok ptoks].
+      * destruct prefix0 as [| ptok' ptoks']; simpl in *.
+        -- subst.
+           apply IHtr in H2; auto.
+           eapply IHtr0 in H6; auto.
+           ++ subst.
+              auto.
+           ++ assert (NT ntName :: tlSyms =
+                      [NT ntName] ++ tlSyms) by auto.
+              rewrite H in Hin.
+              rewrite app_assoc in Hin.
+              eauto.
+           ++ eapply derives_app; eauto.
+              econstructor.
+              eauto.
+              constructor.
+        -- destruct suffix as [| stok stoks].
+           ++ inv H1.
+           ++ inv H1.
+              (* first/follow conflict *)
+              exfalso.
+              
+
+
+
+
+
+
+
+
+              
+              destruct suffix0 as [| stok' stoks']; simpl in *.
+              ** rewrite app_nil_r in *.
+                 assert ((@derivesGamma g) (NT ntName :: tlSyms)
+                                           (stok :: ptoks')
+                                           (Fcons hdTree tlTrees)).
+                 { assert (stok :: ptoks' =
+                           stok :: ptoks' ++ []).
+                   { rewrite app_nil_r.
+                     auto. }
+                   rewrite H.
+                   eapply derivesFcons with
+                       (prefix := stok :: ptoks')
+                       (suffix := nil); auto. }
+                 assert ((@derivesGamma g) (NT ntName :: tlSyms)
+                                           (stok :: ptoks')
+                                           (Fcons tr f)).
+                 { assert (stok :: ptoks' =
+                           [] ++ stok :: ptoks') by auto.
+                   rewrite H0.
+                   eapply derivesFcons with
+                       (prefix := nil)
+                       (suffix := stok :: ptoks'); auto. }
+                 apply (derives_app g [NT ntName] tlSyms
+                                    [stok] ptoks' (Fcons hdTree Fnil) tlTrees) in H.
+
+                 
+
+                            
+
+                                           
+                                        
+           
+
+(* I think we need to break gamma into two parts *)
+Lemma derivesSym_det :
+  forall tbl g,
+    isParseTableFor tbl g
+    -> forall tr tr' sym tokens,
+      (@derivesSym g) sym tokens tr
+      -> (@derivesSym g) sym tokens tr'
+      -> tr = tr'.
+Proof.
+  intros tbl g Htbl.
+  induction tr using tree_mutual_ind with
+      (P := fun tr =>
+              forall tr' sym tokens,
+                (@derivesSym g) sym tokens tr
+                -> (@derivesSym g) sym tokens tr'
+                -> tr = tr')
+      (P0 := fun fSuf =>
+               forall fSuf' fPre x gamma tokens,
+                 In (x, gamma) (productions g)
+                 -> (@derivesGamma g) gamma
+                                      tokens
+                                      (appF fPre fSuf)
+                 -> (@derivesGamma g) gamma
+                                      tokens
+                                      (appF fPre fSuf')
+                 -> fSuf = fSuf').
+
+  - intros tr' sym tokens Hder Hder'.
+    inv Hder.
+    + inv Hder'.
+      auto.
+    + inv H.
+
+  - intros tr' sym tokens Hder Hder'.
+    inv Hder; inv Hder'.
+    inv H; inv H1.
+    pose proof H7 as Hder.
+    pose proof H0 as Hder'.
+    rename s into x.
+    destruct Htbl as [Hmin Hcom].
+    destruct tokens as [| tok toks].
+    + apply derivesGamma_nil_nullable in Hder.
+      apply derivesGamma_nil_nullable in Hder'.
+      assert (Hlk : (@isLookaheadFor g) EOF x gamma).
+      { unfold isLookaheadFor.
+        right.
+        split.
+        - constructor; auto.
+        - constructor; auto.
+          repeat (econstructor; eauto). }
+      assert (Hlk' : (@isLookaheadFor g) EOF x gamma0).
+      { unfold isLookaheadFor.
+        right.
+        split.
+        - constructor; auto.
+        - constructor; auto.
+          repeat (econstructor; eauto). }
+      unfold ptComplete in Hcom.
+      apply Hcom in Hlk.
+      apply Hcom in Hlk'.
+      destruct Hlk as [laMap [Hsf Hlf]].
+      destruct Hlk' as [laMap' [Hsf' Hlf']].
+      assert (gamma = gamma0) by congruence.
+      subst.
+      erewrite IHtr; eauto.
+      * rewrite <- appF_nil_l in H7.
+        eauto.
+      * rewrite <- appF_nil_l in H0.
+        auto.
+    + apply derivesGamma_cons_firstGamma in Hder.
+      apply derivesGamma_cons_firstGamma in Hder'.
+      assert (Hlk : (@isLookaheadFor g) (LA tok) x gamma).
+      { unfold isLookaheadFor.
+        left.
+        constructor; auto. }
+      assert (Hlk' : (@isLookaheadFor g) (LA tok) x gamma0).
+      { unfold isLookaheadFor.
+        left.
+        constructor; auto. }
+      unfold ptComplete in Hcom.
+      apply Hcom in Hlk.
+      apply Hcom in Hlk'.
+      destruct Hlk as [laMap [Hsf Hlf]].
+      destruct Hlk' as [laMap' [Hsf' Hlf']].
+      assert (gamma = gamma0) by congruence.
+      subst.
+      erewrite IHtr; eauto.
+      * rewrite <- appF_nil_l in H7.
+        eauto.
+      * rewrite <- appF_nil_l in H0.
+        auto.
+
+  - intros fSuf' fPre x gamma tokens Hin Hder Hder'.
+    rewrite appF_nil_r in Hder.
+    destruct fSuf'.
+    + auto.
+    + exfalso.
+      apply forest_length in Hder.
+      apply forest_length in Hder'.
+      rewrite Hder in Hder'.
+      apply lengths_contra in Hder'.
+      inv Hder'.
+
+  - intros fSuf' fPre x gamma tokens Hin Hder Hder'.
+    inv Hder; inv Hder'.
+    + exfalso.
+      eapply appF_Fcons_not_Fnil.
+      eauto.
+    + destruct hdSym as [tName | ntName].
+      * inv H0.
+        inv H6.
+        inv H4.
+        assert ((@derivesGamma g) (T tName :: tlSyms)
+                                  (tName :: suffix)
+                                  (Fcons (Leaf tName) tlTrees)).
+        { eapply derivesFcons with (prefix := [tName]).
+          { constructor. }
+          { auto. }}
+        assert ((@derivesGamma g) (T tName :: tlSyms)
+                                  (tName :: suffix)
+                                  (Fcons (Leaf tName) tlTrees0)).
+        { eapply derivesFcons with (prefix := [tName]).
+          { constructor. }
+          { auto. }}
+        rewrite H in H0.
+        assert (Fcons (Leaf tName) tlTrees0 =
+                appF (Fcons (Leaf tName) Fnil) tlTrees0).
+        { simpl. auto. }
+        rewrite H2 in H1.
+        clear H2.
+        eapply IHtr0 in H1.
+        -- subst.
+           inv H0.
+           
+        assert (appF fPre (Fcons tr f) =
+                appF (appF fPre (Fcons tr Fnil)) f).
+        { admit. }
+        rewrite H0 in H.
+        
+
+      
+          
+Lemma derivesSym_det :
+  forall tbl g,
+    isParseTableFor tbl g
+    -> forall tr tr' sym tokens,
+      (@derivesSym g) sym tokens tr
+      -> (@derivesSym g) sym tokens tr'
+      -> tr = tr'.
+Proof.
+  intros tbl g Htbl.
+  induction tr using tree_mutual_ind with
+      (P := fun tr =>
+              forall tr' sym tokens,
+                (@derivesSym g) sym tokens tr
+                -> (@derivesSym g) sym tokens tr'
+                -> tr = tr')
+      (* maybe say something about what gammaPrefix derives *)
+      (P0 := fun f =>
+               forall f' x gammaPrefix gamma tokens,
+                 In (x, gammaPrefix ++ gamma) (productions g)
+                 -> (@derivesGamma g) gamma tokens f
+                 -> (@derivesGamma g) gamma tokens f'
+                 -> f = f').
+
+  - intros tr' sym tokens Hder Hder'.
+    inv Hder; inv Hder'.
+    + auto.
+    + inv H.
+
+  - intros tr' sym tokens Hder Hder'.
+    inv Hder; inv Hder'.
+    inv H; inv H1.
+    pose proof H7 as Hder.
+    pose proof H0 as Hder'.
+    rename s into x.
+    destruct Htbl as [Hmin Hcom].
+    destruct tokens as [| tok toks].
+    + apply derivesGamma_nil_nullable in Hder.
+      apply derivesGamma_nil_nullable in Hder'.
+      assert (Hlk : (@isLookaheadFor g) EOF x gamma).
+      { unfold isLookaheadFor.
+        right.
+        split.
+        - constructor; auto.
+        - constructor; auto.
+          repeat (econstructor; eauto). }
+      assert (Hlk' : (@isLookaheadFor g) EOF x gamma0).
+      { unfold isLookaheadFor.
+        right.
+        split.
+        - constructor; auto.
+        - constructor; auto.
+          repeat (econstructor; eauto). }
+      unfold ptComplete in Hcom.
+      apply Hcom in Hlk.
+      apply Hcom in Hlk'.
+      destruct Hlk as [laMap [Hsf Hlf]].
+      destruct Hlk' as [laMap' [Hsf' Hlf']].
+      assert (gamma = gamma0) by congruence.
+      subst.
+      erewrite IHtr; eauto.
+      assert (gamma0 = [] ++ gamma0) by auto.
+      rewrite H1 in H.
+      eauto.
+
+    + apply derivesGamma_cons_firstGamma in Hder.
+      apply derivesGamma_cons_firstGamma in Hder'.
+      assert (Hlk : (@isLookaheadFor g) (LA tok) x gamma).
+      { unfold isLookaheadFor.
+        left.
+        constructor; auto. }
+      assert (Hlk' : (@isLookaheadFor g) (LA tok) x gamma0).
+      { unfold isLookaheadFor.
+        left.
+        constructor; auto. }
+      unfold ptComplete in Hcom.
+      apply Hcom in Hlk.
+      apply Hcom in Hlk'.
+      destruct Hlk as [laMap [Hsf Hlf]].
+      destruct Hlk' as [laMap' [Hsf' Hlf']].
+      assert (gamma = gamma0) by congruence.
+      subst.
+      erewrite IHtr; eauto.
+      assert (gamma0 = [] ++ gamma0) by auto.
+      rewrite H1 in H.
+      eauto.
+
+  - intros f' x gammaPrefix gamma tokens Hin Hder Hder'.
+    inv Hder; inv Hder'.
+    auto.
+
+  - intros f' x gammaPrefix gamma tokens Hin Hder Hder'.
+    inv Hder; inv Hder'.
+    destruct hdSym as [tName | ntName].
+    + inv H2.
+      inv H3.
+      inv H1.
+      eapply IHtr0 in H6; subst; eauto.
+      assert (T tName :: tlSyms = [T tName] ++ tlSyms) by auto.
+      rewrite H in Hin.
+      rewrite app_assoc in Hin.
+      eauto.
+    + destruct Htbl as [Hmin Hcom].
+      destruct prefix as [| ptok ptoks].
+      * destruct prefix0 as [| ptok' ptoks']; simpl in *.
+        -- (* prefix is nil, prefix0 is nil *)
+          subst.
+          apply IHtr in H2; auto.
+          eapply IHtr0 in H6; eauto.
+          ++ subst.
+             auto.
+          ++ assert (NT ntName :: tlSyms =
+                     [NT ntName] ++ tlSyms) by auto.
+             rewrite H in Hin.
+             rewrite app_assoc in Hin.
+             eauto.
+        -- (* prefix is nil, prefix0 is ptok' :: ptoks' *)
+          destruct suffix as [| stok stoks].
+          ++ inv H1.
+          ++ 
+Abort.
+
+Lemma derivesProd_det :
+  forall tbl g,
+    isParseTableFor tbl g
+    -> forall tr tr' x gamma tokens,
+      (@derivesProd g) x gamma tokens tr
+      -> (@derivesProd g) x gamma tokens tr'
+      -> tr = tr'.
+Proof.
+  intros tbl g Htbl.
+  induction tr using tree_mutual_ind with
+      (P := fun tr =>
+              forall tr' x gamma tokens,
+                (@derivesProd g) x gamma tokens tr
+                -> (@derivesProd g) x gamma tokens tr'
+                -> tr = tr')
+      (P0 := fun f =>
+               forall f' x gammaPrefix gamma tokens,
+                 In (x, gammaPrefix ++ gamma) (productions g)
+                 -> (@derivesGamma g) gamma tokens f
+                 -> (@derivesGamma g) gamma tokens f'
+                 -> f = f').
+
+  - intros tr' x gamma tokens Hder Hder'.
+    inv Hder.
+
+  - intros tr' x gamma tokens Hder Hder'.
+    inv Hder.
+    inv Hder'.
+    erewrite IHtr; eauto.
+    assert (gamma = [] ++ gamma) by auto.
+    rewrite H1 in H.
+    eauto.
+
+  - intros f' x gammaPrefix gamma tokens Hin Hder Hder'.
+    inv Hder.
+    inv Hder'.
+    auto.
+
+  - intros f' x gammaPrefix gamma tokens Hin Hder Hder'.
+    inv Hder.
+    inv Hder'.
+    destruct hdSym as [tName | ntName].
+    + inv H2.
+      inv H3.
+      inv H1.
+      eapply IHtr0 in H6; subst; eauto.
+      assert (T tName :: tlSyms = [T tName] ++ tlSyms) by auto.
+      rewrite H in Hin.
+      rewrite app_assoc in Hin.
+      eauto.
+    + destruct Htbl as [Hmin Hcom].
+      inv H2.
+      inv H3.
+      inv H0.
+      inv H2.
+      destruct prefix as [| ptok ptoks].
+      * destruct prefix0 as [| ptok' ptoks']; simpl in *.
+        -- (* prefix is nil, suffix is nil *)
+          pose proof H3 as Hder.
+          pose proof H5 as Hder'.
+          apply derivesGamma_nil_nullable in H3.
+          apply derivesGamma_nil_nullable in H5.
+          assert (Hlk : (@isLookaheadFor g) EOF ntName gamma).
+          { unfold isLookaheadFor.
+            right.
+            split.
+            - constructor; auto.
+            - constructor; auto.
+              repeat (econstructor; eauto). }
+          assert (Hlk' : (@isLookaheadFor g) EOF ntName gamma0).
+          { unfold isLookaheadFor.
+            right.
+            split.
+            - constructor; auto.
+            - constructor; auto.
+              repeat (econstructor; eauto). }
+          unfold ptComplete in Hcom.
+          apply Hcom in Hlk.
+          apply Hcom in Hlk'.
+          destruct Hlk as [laMap [Hsf Hlf]].
+          destruct Hlk' as [laMap' [Hsf' Hlf']].
+          assert (gamma = gamma0) by congruence.
+          subst.
+          assert ((@derivesProd g) ntName
+                                   gamma0
+                                   []
+                                   (Node ntName f0))
+            by repeat (constructor; auto).
+          assert ((@derivesProd g) ntName
+                                   gamma0
+                                   []
+                                   (Node ntName f1))
+            by repeat (constructor; auto).
+          apply IHtr in H1; auto.
+          inv H1.
+          eapply IHtr0 in H6; eauto.
+          ++ subst; auto.
+          ++ assert (NT ntName :: tlSyms =
+                     [NT ntName] ++ tlSyms) by auto.
+             rewrite H1 in Hin.
+             rewrite app_assoc in Hin.
+             eauto.
+        -- (* prefix is nil, prefix0 is cons *)
+          destruct suffix as [| stok stoks].
+          ++ inv H1.
+          ++ (* [] ++ (stok :: stoks) = 
+                (ptok' :: ptoks') ++ suf0
+
+                stok :: stoks = ptok' :: ptoks' *)
+            symmetry in H1.
+            inv H1.
+            assert (Hlk : (@isLookaheadFor g) (LA ptok')
+                                              ntName
+                                              gamma).
+            { unfold isLookaheadFor.
+              left.
+              constructor; auto.
+              apply derivesGamma_cons_firstGamma in H3.
+              auto. }
+            assert (Hlk' : (@isLookaheadFor g) (LA ptok')
+                                               ntName
+                                               gamma0).
+            { unfold isLookaheadFor.
+              right.
+              split.
+              { constructor; auto.
+                apply derivesGamma_nil_nullable in H5.
+                auto. }
+              { constructor; auto.
+                eapply FoRight; eauto.
+                apply derivesGamma_cons_firstGamma in H4.
+                auto. }}
+            unfold ptComplete in Hcom.
+            apply Hcom in Hlk; apply Hcom in Hlk'.
+            destruct Hlk as [laMap [Hsf Hlf]].
+            destruct Hlk' as [laMap' [Hsf' Hlf']].
+            assert (gamma = gamma0) by congruence.
+            subst.
+            clear Hsf Hsf' Hlf Hlf' laMap laMap'.
+            (* looking good -- we've reached a first/follow
+               conflict, but I don't think that's quite 
+               enough to finish. Maybe try switching the
+               proof from derivesProd to derivesSym *)
+            
+            
+      
+ 
+Lemma derivesProd_det :
+  forall tbl g x gamma tokens tr,
+    isParseTableFor tbl g
+    -> (@derivesProd g) x gamma tokens tr
+    -> forall tr',
+        (@derivesProd g) x gamma tokens tr'
+        -> tr = tr'.
+Proof.
+  intros tbl g x gamma tokens tr Htbl Hder.
+  induction Hder using derivesProd_mutual_ind with
+      (P := fun x gamma tokens tr
+                (pf : (@derivesProd g) x gamma tokens tr) =>
+              forall tr',
+                (@derivesProd g) x gamma tokens tr'
+                -> tr = tr')
+      (P0 := fun sym tokens tr
+                 (pf : (@derivesSym g) sym tokens tr) =>
+               forall tr',
+                 (@derivesSym g) sym tokens tr'
+                 -> tr = tr')
+      (P1 := fun gamma tokens f
+                 (pf : (@derivesGamma g) gamma tokens f) =>
+               forall x gammaPrefix f',
+                 In (x, gammaPrefix ++ gamma) (productions g)
+                 -> (@derivesGamma g) gamma tokens f'
+                 -> f = f').
+
+  - intros tr' Hder.
+    inv Hder.
+    apply (IHHder x nil f0) in H0; subst; auto.
+    
+  - intros tr' Hder.
+    inv Hder.
+    auto.
+
+  - intros tr' Hder'.
+    inv Hder.
+    inv Hder'.
+    inv H2.
+    pose proof H0 as Hder.
+    pose proof H3 as Hder'.
+    destruct Htbl as [Hmin Hcom].
+    destruct tokens as [| tok toks].
+    + apply derivesGamma_nil_nullable in Hder.
+      apply derivesGamma_nil_nullable in Hder'.
+      assert (Hlk : (@isLookaheadFor g) EOF x gamma).
+      { unfold isLookaheadFor.
+        right.
+        split.
+        - constructor; auto.
+        - constructor; auto.
+          repeat (econstructor; eauto). }
+      assert (Hlk' : (@isLookaheadFor g) EOF x gamma0).
+      { unfold isLookaheadFor.
+        right.
+        split.
+        - constructor; auto.
+        - constructor; auto.
+          repeat (econstructor; eauto). }
+      unfold ptComplete in Hcom.
+      apply Hcom in Hlk.
+      apply Hcom in Hlk'.
+      destruct Hlk as [laMap [Hsf Hlf]].
+      destruct Hlk' as [laMap' [Hsf' Hlf']].
+      assert (gamma = gamma0) by congruence.
+      subst.
+      apply IHHder.
+      constructor; auto.
+    + apply derivesGamma_cons_firstGamma in Hder.
+      apply derivesGamma_cons_firstGamma in Hder'.
+      assert (Hlk : (@isLookaheadFor g) (LA tok) x gamma).
+      { unfold isLookaheadFor.
+        left.
+        constructor; auto. }
+      assert (Hlk' : (@isLookaheadFor g) (LA tok) x gamma0).
+      { unfold isLookaheadFor.
+        left.
+        constructor; auto. }
+      unfold ptComplete in Hcom.
+      apply Hcom in Hlk.
+      apply Hcom in Hlk'.
+      destruct Hlk as [laMap [Hsf Hlf]].
+      destruct Hlk' as [laMap' [Hsf' Hlf']].
+      assert (gamma = gamma0) by congruence.
+      subst.
+      apply IHHder.
+      constructor; auto.
+
+  - intros x gammaPrefix f' Hin Hder.
+    inv Hder.
+    auto.
+
+  - intros x gammaPrefix f' Hin Hder.
+    inv Hder.
+    assert (Heq : gammaPrefix ++ hdSym :: tlSyms =
+            gammaPrefix ++ [hdSym] ++ tlSyms) by auto.
+    rewrite Heq in Hin.
+    rewrite app_assoc in Hin.
+    destruct hdSym as [tName | ntName].
+    + inv d; inv H2.
+      inv H1.
+      apply IHHder0 with
+          (x := x)
+          (gammaPrefix := app gammaPrefix [T tName])
+          (f' := tlTrees0) in Hin; auto.
+      subst.
+      auto.
+    + destruct prefix as [| ptok ptoks];
+        destruct prefix0 as [| ptok' ptoks']; simpl in *.
+
+      * (* prefix and prefix0 are nil *)
+        subst.
+        apply IHHder in H2.
+        subst.
+        apply IHHder0 with
+            (x := x)
+            (gammaPrefix := app gammaPrefix [NT ntName])
+            (f' := tlTrees0) in Hin; auto.
+        subst; auto.
+      * (* prefix is nil, prefix0 is cons *)
+        (* we should be able to get a first/follow contra? *)
+        destruct suffix as [| stok stoks];
+          destruct suffix0 as [| stok' stoks']; simpl in *.
+        -- inv H1.
+        -- inv H1. 
+        -- inv H1.
+           rewrite app_nil_r in *.
+           inv H2.
+           inv H0.
+           assert (Hlk : (@isLookaheadFor g) (LA stok) ntName gamma).
+           { unfold isLookaheadFor.
+             left.
+             constructor; auto.
+             apply derivesGamma_cons_firstGamma in H1.
+             auto. }
+           inv d.
+           inv H2.
+           assert (Hlk' : (@isLookaheadFor g) (LA stok) ntName gamma0).
+           { unfold isLookaheadFor.
+             right.
+             split.
+             { constructor; auto.
+               apply derivesGamma_nil_nullable in H3; auto. }
+             { constructor; auto.
+               eapply FoRight.
+               { (* hmm, Heq got corrupted somehow *)
+                 assert ([NT ntName] ++ tlSyms =
+                         NT ntName :: tlSyms) by auto.
+                 rewrite <- app_assoc in Hin.
+                 rewrite H2 in Hin.
+                 eauto. }
+               { apply derivesGamma_cons_firstGamma in d0.
+                 auto. }}}
+           destruct Htbl as [Hmin Hcom].
+           unfold ptComplete in Hcom.
+           apply Hcom in Hlk.
+           apply Hcom in Hlk'.
+           destruct Hlk as [laMap [Hsf Hlf]].
+           destruct Hlk' as [laMap' [Hsf' Hlf']].
+           assert (Hgammas : gamma = gamma0) by congruence.
+           subst.
+           clear Hsf; clear Hlf; clear Hsf'; clear Hlf'.
+           clear laMap; clear laMap'.
+Abort. (* seems promising, but I think the induction has
+          to be more general *)
+
+Lemma derivesProd_det :
+  forall tbl g x gamma tokens tr,
+    isParseTableFor tbl g
+    -> (@derivesProd g) x gamma tokens tr
+    -> forall tr',
+        (@derivesProd g) x gamma tokens tr'
+        -> tr = tr'.
+Proof.
+  intros tbl g x gamma tokens tr Htbl Hder.
+  induction Hder using derivesProd_mutual_ind with
+      (P := fun x gamma tokens tr
+                (pf : (@derivesProd g) x gamma tokens tr) =>
+              forall tr',
+                (@derivesProd g) x gamma tokens tr'
+                -> tr = tr')
+      (P0 := fun sym tokens tr
+                 (pf : (@derivesSym g) sym tokens tr) =>
+               forall tr',
+                 (@derivesSym g) sym tokens tr'
+                 -> tr = tr')
+      (P1 := fun gamma tokens f
+                 (pf : (@derivesGamma g) gamma tokens f) =>
+               forall f',
+                 (@derivesGamma g) gamma tokens f'
+                 -> f = f').
+  
+  - intros tr' Hder.
+    inv Hder.
+    apply IHHder in H0; auto.
+    subst.
+    auto.
+    
+  - intros tr' Hder.
+    inv Hder.
+    auto.
+
+  - intros tr' Hder'.
+    inv Hder.
+    inv Hder'.
+    inv H2.
+    pose proof H0 as Hder.
+    pose proof H3 as Hder'.
+    destruct Htbl as [Hmin Hcom].
+    destruct tokens as [| tok toks].
+    + apply derivesGamma_nil_nullable in Hder.
+      apply derivesGamma_nil_nullable in Hder'.
+      assert (Hlk : (@isLookaheadFor g) EOF x gamma).
+      { unfold isLookaheadFor.
+        right.
+        split.
+        - constructor; auto.
+        - constructor; auto.
+          repeat (econstructor; eauto). }
+      assert (Hlk' : (@isLookaheadFor g) EOF x gamma0).
+      { unfold isLookaheadFor.
+        right.
+        split.
+        - constructor; auto.
+        - constructor; auto.
+          repeat (econstructor; eauto). }
+      unfold ptComplete in Hcom.
+      apply Hcom in Hlk.
+      apply Hcom in Hlk'.
+      destruct Hlk as [laMap [Hsf Hlf]].
+      destruct Hlk' as [laMap' [Hsf' Hlf']].
+      assert (gamma = gamma0) by congruence.
+      subst.
+      apply IHHder.
+      constructor; auto.
+    + apply derivesGamma_cons_firstGamma in Hder.
+      apply derivesGamma_cons_firstGamma in Hder'.
+      assert (Hlk : (@isLookaheadFor g) (LA tok) x gamma).
+      { unfold isLookaheadFor.
+        left.
+        constructor; auto. }
+      assert (Hlk' : (@isLookaheadFor g) (LA tok) x gamma0).
+      { unfold isLookaheadFor.
+        left.
+        constructor; auto. }
+      unfold ptComplete in Hcom.
+      apply Hcom in Hlk.
+      apply Hcom in Hlk'.
+      destruct Hlk as [laMap [Hsf Hlf]].
+      destruct Hlk' as [laMap' [Hsf' Hlf']].
+      assert (gamma = gamma0) by congruence.
+      subst.
+      apply IHHder.
+      constructor; auto.
+
+  - intros f' Hder.
+    inv Hder.
+    auto.
+
+  - intros f' Hder. 
+    inv Hder.
+Abort.
+(* The problem here is that we don't know that (hdSym :: tlSyms) is the RHS of some production in the grammar, so we probably
+  won't be able to prove that prefix = prefix0, hdTree = tr',
+  etc. *)
